incomplete proof for version with 'visited successors' component

Isabelle/Graph.thy
@@ -13,6 +13,7 @@ record 'v env =
   \<S> :: "'v \<Rightarrow> 'v set"
   explored :: "'v set"
   visited :: "'v set"
+  vsuccs :: "'v \<Rightarrow> 'v set"
   sccs :: "'v set set"
   stack :: "'v list"
 
@@ -257,70 +258,52 @@ qed
 
 text \<open>
   We also need the following variant of reachability avoiding
-  some node. More precisely, @{text y} is reachable from @{text x}
-  avoiding @{text S} if there exists a path such that no node from
-  @{text S} appears along the path, except possibly as the start
-  node.
+  certain edges. More precisely, @{text y} is reachable from @{text x}
+  avoiding @{text E} if there exists a path such that no edge from
+  @{text E} appears along the path.
 \<close>
 inductive reachable_avoiding where
-  ra_refl[iff]: "reachable_avoiding x x S"
-| ra_succ[elim]: "\<lbrakk>reachable_avoiding x y S; edge y z; z \<notin> S\<rbrakk> \<Longrightarrow> reachable_avoiding x z S"
+  ra_refl[iff]: "reachable_avoiding x x E"
+| ra_succ[elim]: "\<lbrakk>reachable_avoiding x y E; edge y z; (y,z) \<notin> E\<rbrakk> \<Longrightarrow> reachable_avoiding x z E"
 
 lemma edge_ra:
-  assumes "edge x y" and "y \<notin> S"
-  shows "reachable_avoiding x y S"
+  assumes "edge x y" and "(x,y) \<notin> E"
+  shows "reachable_avoiding x y E"
   using assms by (meson reachable_avoiding.simps)
 
 lemma ra_trans:
-  assumes 1: "reachable_avoiding x y S" and 2: "reachable_avoiding y z S"
-  shows "reachable_avoiding x z S"
+  assumes 1: "reachable_avoiding x y E" and 2: "reachable_avoiding y z E"
+  shows "reachable_avoiding x z E"
   using 2 1 by induction auto
 
 lemma ra_cases:
-  assumes "reachable_avoiding x y S"
-  shows "x=y \<or> (\<exists>z. z \<in> successors x - {x} \<and> z \<notin> S \<and> reachable_avoiding z y S)"
+  assumes "reachable_avoiding x y E"
+  shows "x=y \<or> (\<exists>z. z \<in> successors x \<and> (x,z) \<notin> E \<and> reachable_avoiding z y E)"
 using assms proof (induction)
   case (ra_refl x S)
   then show ?case by simp
 next
   case (ra_succ x y S z)
   then show ?case
-    by (metis DiffI emptyE insert_iff ra_refl reachable_avoiding.ra_succ)
+    by (metis ra_refl reachable_avoiding.ra_succ)
 qed
 
 lemma ra_mono: 
-  assumes "reachable_avoiding x y S" and "S' \<subseteq> S"
-  shows "reachable_avoiding x y S'"
+  assumes "reachable_avoiding x y E" and "E' \<subseteq> E"
+  shows "reachable_avoiding x y E'"
 using assms by induction auto
 
 text \<open>
-  Reachability avoiding some nodes obviously implies reachability.
-  Conversely, if @{text y} is reachable from @{text "x \<in> S"} then there
-  exists some @{text "x' \<in> S"} from which @{text y} can be reached
-  without (again) passing through @{text S}.
+  Reachability avoiding some edges obviously implies reachability.
+  Conversely, reachability implies reachability avoiding the empty set.
 \<close>
 lemma ra_reachable:
-  "reachable_avoiding x y S \<Longrightarrow> reachable x y"
+  "reachable_avoiding x y E \<Longrightarrow> reachable x y"
   by (induction rule: reachable_avoiding.induct) (auto intro: succ_reachable)
 
-lemma reach_avoid:
-  assumes r: "reachable x y" and x: "x \<in> S"
-  shows "\<exists>x'\<in>S. reachable_avoiding x' y S"
-  using r[THEN reachable_re] x proof (induction)
-  case (re_refl x)
-  then show ?case by auto
-next
-  case (re_succ x y z)
-  show ?case 
-  proof (cases "z \<in> S")
-    case True
-    then show ?thesis by auto
-  next
-    case False
-    with re_succ ra_succ show ?thesis by blast
-  qed
-qed
-
+lemma ra_empty:
+  "reachable_avoiding x y {} = reachable x y"
+  sorry
 
 section \<open>Strongly connected components\<close>
 
@@ -350,6 +333,7 @@ lemma scc_partition:
   using assms unfolding is_scc_def is_subscc_def
   by (metis IntE assms(2) sccE subsetI)
 
+
 section \<open>Algorithm for computing strongly connected components\<close>
 
 (*
@@ -372,22 +356,36 @@ definition unite :: "'v \<Rightarrow> 'v \<Rightarrow> 'v env \<Rightarrow> 'v e
      in  e\<lparr>\<S> := \<lambda>x. if x \<in> cc then cc else \<S> e x,
            stack := sfx\<rparr>"
 
-function dfs :: "'v \<Rightarrow> 'v env \<Rightarrow> 'v env" and dfss :: "'v \<Rightarrow> 'v set \<Rightarrow> 'v env \<Rightarrow> 'v env" where
+function dfs :: "'v \<Rightarrow> 'v env \<Rightarrow> 'v env" and dfss :: "'v \<Rightarrow> 'v env \<Rightarrow> 'v env" where
   "dfs v e =
   (let e1 = e\<lparr>visited := visited e \<union> {v}, stack := (v # stack e)\<rparr>;
-       e' = dfss v (successors v) e1
-  in if v = hd(stack e')
-      then e'\<lparr>sccs:=sccs e' \<union> {\<S> e' v}, explored:=explored e' \<union> (\<S> e' v), stack:=tl(stack e')\<rparr>
-    else e')"
-| "dfss v vs e =
-   (if vs = {} then e
-   else (let w = SOME x. x \<in> vs
-     in (let e' = (if w \<in> explored e then e
+       e' = dfss v e1
+   in if v = hd(stack e')
+      then e'\<lparr>sccs := sccs e' \<union> {\<S> e' v}, 
+              explored := explored e' \<union> (\<S> e' v), 
+              stack := tl(stack e')\<rparr>
+      else e')"
+| "dfss v e =
+   (let vs = successors v - vsuccs e v
+    in  if vs = {} then e
+        else let w = SOME x. x \<in> vs;
+                 e' = (if w \<in> explored e then e
                        else if w \<notin> visited e
                        then dfs w e
-                       else unite v w e)
-          in dfss v (vs-{w}) e')))"
+                       else unite v w e);
+                 e'' = (e'\<lparr>vsuccs := 
+                             (\<lambda>x. if x=v then vsuccs e' v \<union> {w} 
+                                  else vsuccs e' x)\<rparr>)
+             in  dfss v e'')"
   by pat_completeness (force+)
+
+text \<open>
+  Set of edges starting from some node in the
+  equivalence class of node that have not yet been followed.
+\<close>
+definition unvisited where
+  "unvisited e x \<equiv> 
+   {(a,b) | a b. a \<in> \<S> e x \<and> b \<in> successors a - vsuccs e a}"
 
 text \<open>
   Well-formed environments.
@@ -398,6 +396,10 @@ definition wf_env where
   \<and> set (stack e) \<subseteq> visited e
   \<and> explored e \<subseteq> visited e
   \<and> explored e \<inter> set (stack e) = {}
+  \<and> (\<forall>v. vsuccs e v \<subseteq> successors v)
+  \<and> (\<forall>v. vsuccs e v \<subseteq> visited e)
+  \<and> (\<forall>v. v \<notin> visited e \<longrightarrow> vsuccs e v = {})
+  \<and> (\<forall>v. v \<in> explored e \<longrightarrow> vsuccs e v = successors v)
   \<and> (\<forall>v w. w \<in> \<S> e v \<longleftrightarrow> (\<S> e v = \<S> e w))
   \<and> (\<forall>v \<in> set (stack e). \<forall> w \<in> set (stack e). v \<noteq> w \<longrightarrow> \<S> e v \<inter> \<S> e w = {})
   \<and> (\<forall> v. v \<notin> visited e \<longrightarrow> \<S> e v = {v})
@@ -406,16 +408,27 @@ definition wf_env where
   \<and> (\<forall> x. is_subscc (\<S> e x))
   \<and> (\<forall> x \<in> explored e. \<forall> y. reachable x y \<longrightarrow> y \<in> explored e)  
   \<and> (\<forall> S \<in> sccs e. is_scc S)
+  \<and> (\<forall>x y. x \<preceq> y in stack e \<and> x \<noteq> y \<longrightarrow>
+        (\<forall>u \<in> \<S> e x. \<not> reachable_avoiding u y (unvisited e x)))
 "
+(*
+  \<and> (\<forall>v w x. w \<in> vsuccs e v \<and> reachable w x \<longrightarrow> 
+             vsuccs e x = successors x) 
+*)
 
 definition sub_env where
   "sub_env e e' \<equiv> visited e \<subseteq> visited e'
                 \<and> explored e \<subseteq> explored e'
+                \<and> (\<forall>v. vsuccs e v \<subseteq> vsuccs e' v)
                 \<and> (\<forall> v. \<S> e v \<subseteq> \<S> e' v)
                 \<and> (\<Union> {\<S> e v | v . v \<in> set (stack e)})
                    \<subseteq> (\<Union> {\<S> e' v | v . v \<in> set (stack e')})
 "
 
+lemma sub_env_trans:
+  assumes "sub_env e e'" and "sub_env e' e''"
+  shows "sub_env e e''"
+  using assms unfolding sub_env_def by (meson subset_eq)
 
 text \<open>
   Precondition and post-condition for function dfs.
@@ -424,20 +437,23 @@ definition pre_dfs where
   "pre_dfs v e \<equiv> 
      wf_env e
    \<and> v \<notin> visited e
-   \<and> (\<forall> n \<in> set (stack e). reachable n v)"
+   \<and> vsuccs e v = {}
+   \<and> (\<forall>n \<in> set (stack e). reachable n v)"
 
 definition post_dfs where 
   "post_dfs v prev_e e \<equiv> 
      wf_env e
-   \<and> (\<forall> x. reachable v x \<longrightarrow> x \<in> visited e)
+   \<and> v \<in> visited e
+   \<and> (\<forall>x. reachable v x \<longrightarrow> 
+          x \<in> visited e \<or> (\<exists>n \<in> set (tl (stack e)). reachable v n \<and> reachable n x))
    \<and> sub_env prev_e e
-   \<and> (\<forall> n \<in> set (stack e). reachable n v)
-   \<and> (\<exists> ns. stack prev_e = ns @ (stack e))
+   \<and> vsuccs e v = successors v
+   \<and> (\<forall>w \<in> visited prev_e. vsuccs e w = vsuccs prev_e w)
+   \<and> (\<forall>n \<in> set (stack e). reachable n v)
+   \<and> (\<exists>ns. stack prev_e = ns @ (stack e))
    \<and> ((v \<in> explored e \<and> stack e = stack prev_e \<and> (\<forall>n \<in> set (stack e). \<S> e n = \<S> prev_e n)) 
        \<or> (stack e \<noteq> [] \<and> v \<in> \<S> e (hd (stack e)) 
-          \<and> (\<forall>n \<in> set (tl (stack e)). \<S> e n = \<S> prev_e n))
-          \<and> (\<forall>n \<in> set (tl (stack e)). \<forall>w \<in> \<S> e (hd (stack e)) - \<S> prev_e (hd (stack e)).
-                \<not> reachable_avoiding w n (\<S> e (hd (stack e)))))
+          \<and> (\<forall>n \<in> set (tl (stack e)). \<S> e n = \<S> prev_e n)))
 "
 (*
    \<and> ((v \<in> explored e \<and> stack e = stack prev_e)
@@ -451,17 +467,13 @@ text \<open>
   Precondition for function dfss.
 \<close>
 definition pre_dfss where 
-  "pre_dfss v vs e \<equiv> 
+  "pre_dfss v e \<equiv> 
      wf_env e 
    \<and> v \<in> visited e
-   \<and> vs \<subseteq> successors v
-   \<and> (\<forall>w \<in> successors v - vs. w \<in> explored e \<union> \<S> e (hd (stack e)))
+   \<and> (\<forall>w \<in> vsuccs e v. w \<in> explored e \<union> \<S> e (hd (stack e)))
    \<and> (\<forall> n \<in> set (stack e). reachable n v)
    \<and> (stack e \<noteq> [])
    \<and> (v \<in> \<S> e (hd (stack e)))
-   \<and> (hd (stack e) = v \<longrightarrow>
-         (\<forall>n \<in> set (tl (stack e)). \<forall>w \<in> \<S> e (hd (stack e)) - {v}.
-             \<not> reachable_avoiding w n (\<S> e (hd (stack e)))))
 "
 (* \<and> (\<forall>n \<in> set (stack e). \<forall>w \<in> successors v - vs. reachable w n \<longrightarrow> w \<in> \<S> e v) *)
 (* \<and> (\<forall> n \<in> set (stack e). reachable v n \<longrightarrow> v \<in> \<S> e n \<or> (\<exists> m \<in> vs. reachable m n)) *) (* wrong *)
@@ -469,22 +481,22 @@ definition pre_dfss where
          \<not> reachable_avoiding w n (\<S> e (hd (stack e)))) *)
 
 definition post_dfss where 
-  "post_dfss v vs prev_e e \<equiv> 
+  "post_dfss v prev_e e \<equiv> 
      wf_env e
-   \<and> (\<forall> w \<in> vs. \<forall> x. reachable w x \<longrightarrow> x \<in> visited e)
+   \<and> vsuccs e v = successors v
+   \<and> (\<forall>w \<in> visited prev_e - {v}. vsuccs e w = vsuccs prev_e w)
    \<and> sub_env prev_e e
+   \<and> (\<forall>x. reachable v x \<longrightarrow> 
+         x \<in> visited e \<or> (\<exists>n \<in> set (tl (stack e)). reachable v n \<and> reachable n x))
    \<and> (\<forall>w \<in> successors v. w \<in> explored e \<union> \<S> e (hd (stack e)))
    \<and> (\<forall> n \<in> set (stack e). reachable n v)
    \<and> (stack e \<noteq> [])
    \<and> (\<exists> ns. stack prev_e = ns @ (stack e))
    \<and> (v \<in> \<S> e (hd (stack e)))
    \<and> (\<forall>n \<in> set (tl (stack e)). \<S> e n = \<S> prev_e n)
-   \<and> (hd (stack e) = v \<longrightarrow>
-         (\<forall>n \<in> set (tl (stack e)). \<forall>w \<in> \<S> e (hd (stack e)) - {v}.
-             \<not> reachable_avoiding w n (\<S> e (hd (stack e)))))
-   \<and> (hd (stack e) = v \<longrightarrow> (\<forall>n \<in> set (tl (stack e)). \<not> reachable v n)) 
+   \<and> (hd (stack e) = v \<longrightarrow> (\<forall>n \<in> set (tl (stack e)). \<not> reachable v n))
 "
-(* \<and> (set (stack e) \<subseteq> set (stack prev_e) \<union> {v})" *) 
+(* \<and> (set (stack e) \<subseteq> set (stack prev_e) \<union> {v})" *)
 (* \<and> (\<forall> w \<in> vs. \<forall> x. reachable w x \<longrightarrow> x \<in> explored e)" *) (* false *)
 (* \<and> (\<forall> n \<in> set (stack e). reachable v n \<longrightarrow> v \<in> \<S> e n) *) (* wrong *)
 (* \<and> (\<forall>n \<in> set (tl (stack e)). \<not> reachable_avoiding v n (\<S> e (hd (stack e)))) *)
@@ -492,18 +504,59 @@ definition post_dfss where
 
 lemma pre_dfs_pre_dfss:
   assumes "pre_dfs v e"
-  shows "pre_dfss v (successors v) (e\<lparr> visited := visited e \<union> {v}, stack := v # stack e\<rparr>)"
-        (is "pre_dfss v ?succs ?e'")
+  shows "pre_dfss v (e\<lparr> visited := visited e \<union> {v}, stack := v # stack e\<rparr>)"
+        (is "pre_dfss v ?e'")
 proof -
-  have 1:"distinct (stack ?e')"
+  have "distinct (stack ?e')"
        "set (stack ?e') \<subseteq> visited ?e'"
        "explored ?e' \<subseteq> visited ?e'"
+       "\<forall>v. vsuccs ?e' v \<subseteq> successors v"
+       "\<forall>v. vsuccs ?e' v \<subseteq> visited ?e'"
+       "\<forall>v. v \<notin> visited ?e' \<longrightarrow> vsuccs ?e' v = {}"
        "explored ?e' \<inter> set (stack ?e') = {}"
        "(\<forall>w z. z \<in> \<S> ?e' w \<longleftrightarrow> (\<S> ?e' w = \<S> ?e' z))"
-       "(\<forall>v \<in> set (stack ?e'). \<forall> w \<in> set (stack ?e'). v \<noteq> w \<longrightarrow> \<S> ?e' v \<inter> \<S> ?e' w = {})"
        "(\<forall> v. v \<notin> visited ?e' \<longrightarrow> \<S> ?e' v = {v})"
     using assms unfolding pre_dfs_def wf_env_def by auto
-  have 2:"\<Union> {\<S> ?e' v | v . v \<in> set (stack ?e')} = visited ?e' - explored ?e'"
+
+  moreover
+  have "(\<forall>v \<in> set (stack ?e'). \<forall> w \<in> set (stack ?e'). v \<noteq> w \<longrightarrow> \<S> ?e' v \<inter> \<S> ?e' w = {})"
+  proof (clarify)
+    fix x y
+    assume asm: "x \<in> set (stack ?e')" "y \<in> set (stack ?e')" "x \<noteq> y"
+    show "\<S> ?e' x \<inter> \<S> ?e' y = {}"
+    proof (cases "x=v")
+      case True
+      with assms have "\<S> ?e' x = {v}"
+        by (auto simp: pre_dfs_def wf_env_def)
+      with True asm assms \<open>\<forall>w z. (z \<in> \<S> ?e' w) \<longleftrightarrow> (\<S> ?e' w = \<S> ?e' z)\<close> 
+      show ?thesis
+        unfolding pre_dfs_def wf_env_def
+        by (smt (verit) disjoint_iff singleton_iff)
+    next
+      case False
+      show ?thesis
+      proof (cases "y = v")
+        case True
+        with assms have "\<S> ?e' y = {v}"
+          by (auto simp: pre_dfs_def wf_env_def)
+        with True asm assms \<open>\<forall>w z. (z \<in> \<S> ?e' w) \<longleftrightarrow> (\<S> ?e' w = \<S> ?e' z)\<close> 
+        show ?thesis
+          unfolding pre_dfs_def wf_env_def
+          by (smt (verit) disjoint_iff singleton_iff)
+      next
+        case False
+        with \<open>x \<noteq> v\<close> assms asm show ?thesis
+          by (auto simp: pre_dfs_def wf_env_def)
+      qed
+    qed
+  qed
+
+  moreover 
+  have "\<forall>u. u \<in> explored ?e' \<longrightarrow> vsuccs ?e' u = successors u"
+    using assms by (auto simp: pre_dfs_def wf_env_def)
+
+  moreover
+  have "\<Union> {\<S> ?e' v | v . v \<in> set (stack ?e')} = visited ?e' - explored ?e'"
   proof -
     have "\<Union> {\<S> ?e' v | v . v \<in> set (stack ?e')} = 
           (\<Union> {\<S> ?e' v | v . v \<in> set (stack e)}) \<union> \<S> e v"
@@ -513,66 +566,41 @@ proof -
     finally show ?thesis .
   qed
 
-  have 3:"\<forall> x y. x \<preceq> y in stack ?e' \<longrightarrow> reachable y x"
+  moreover
+  have "\<forall> x y. x \<preceq> y in stack ?e' \<longrightarrow> reachable y x"
   proof (clarify)
     fix x y
     assume "x \<preceq> y in stack ?e'"
     show "reachable y x"
     proof (cases "x=v")
       assume "x=v"
-      have "\<forall> y. v \<preceq> y in stack ?e' \<longrightarrow> reachable y v"
-      proof (cases "stack e = []")
-        assume "stack e = []"
-        hence "stack ?e' = [v]" by simp
-        thus ?thesis
-          using precedes_mem(2) by fastforce
-      next
-        assume "stack e \<noteq> []"
-        have reach_hd:"reachable (hd (stack e)) v"
-          using assms \<open>stack e \<noteq> []\<close> unfolding pre_dfs_def by force
-        show ?thesis
-        proof (clarify)
-          fix y
-          assume "v \<preceq> y in stack ?e'"
-          show "reachable y v"
-          proof (cases "y = v")
-            assume "y = v"
-            thus ?thesis
-              by blast
-          next
-            assume "y \<noteq> v"
-            hence "y \<in> set(stack e)"
-              using \<open>v \<preceq> y in stack (e\<lparr>visited := visited e \<union> {v}, stack := v # stack e\<rparr>)\<close> precedes_mem(2) by fastforce 
-            hence "hd(stack e) \<preceq> y in stack e"
-              using \<open>stack e \<noteq> []\<close> head_precedes list.exhaust list.sel(1) by metis
-            hence "reachable y (hd(stack e))"
-              using assms by (auto simp: pre_dfs_def wf_env_def)
-            thus ?thesis using reach_hd reachable_trans by blast
-          qed
-        qed
-      qed
-      thus ?thesis
-        using \<open>x = v\<close> \<open>x \<preceq> y in stack ?e'\<close> by blast 
+      with \<open>x \<preceq> y in stack ?e'\<close> assms show ?thesis
+        unfolding pre_dfs_def
+        by (metis insert_iff list.simps(15) precedes_mem(2) reachable_refl select_convs(6) surjective update_convs(6))
     next
       assume "x \<noteq> v"
+      with \<open>x \<preceq> y in stack ?e'\<close>
       have "x \<preceq> y in stack e"
-        using \<open>x \<noteq> v\<close> \<open>x \<preceq> y in stack ?e'\<close> precedes_in_tail by fastforce
-      thus ?thesis
-        using assms by (simp add: pre_dfs_def wf_env_def)
+        by (simp add: precedes_in_tail)
+      with assms show ?thesis
+        by (simp add: pre_dfs_def wf_env_def)
     qed
   qed
 
-  have 4:"\<forall> x. is_subscc (\<S> ?e' x)" using assms
+  moreover
+  have "\<forall> x. is_subscc (\<S> ?e' x)" using assms
     unfolding pre_dfs_def wf_env_def by simp
 
-  have 5:"\<forall> x \<in> explored ?e'. \<forall> y. reachable x y \<longrightarrow> y \<in> explored ?e'"
+  moreover
+  have "\<forall> x \<in> explored ?e'. \<forall> y. reachable x y \<longrightarrow> y \<in> explored ?e'"
   proof -
     have "explored ?e' = explored e" by simp
     then show ?thesis using assms unfolding wf_env_def
       by (simp add: pre_dfs_def wf_env_def) 
   qed
 
-  have 6:"\<forall> S \<in> sccs ?e'. is_scc S"
+  moreover
+  have "\<forall> S \<in> sccs ?e'. is_scc S"
   proof (clarify)
     fix S
     assume asm:"S \<in> sccs ?e'"
@@ -581,11 +609,42 @@ proof -
       using asm pre_dfs_def wf_env_def by blast
   qed
 
-  have wfenv:"wf_env ?e'" using 1 2 3 4 5 6 unfolding wf_env_def
-    by blast
+  moreover
+  have "\<forall>x y. x \<preceq> y in stack ?e' \<and> x \<noteq> y \<longrightarrow>
+           (\<forall>u \<in> \<S> ?e' x. \<not> reachable_avoiding u y (unvisited ?e' x))"
+  proof (clarify)
+    fix x y u
+    assume asm: "x \<preceq> y in stack ?e'" "x \<noteq> y" "u \<in> \<S> ?e' x"
+                "reachable_avoiding u y (unvisited ?e' x)"
+    show "False"
+    proof (cases "x = v")
+      case True
+      with assms \<open>u \<in> \<S> ?e' x\<close> have "u = v" "vsuccs ?e' v = {}"
+        by (auto simp: pre_dfs_def wf_env_def)
+      with \<open>reachable_avoiding u y (unvisited ?e' x)\<close>[THEN ra_cases]
+           True \<open>x \<noteq> y\<close> assms
+      show ?thesis
+        by (auto simp: pre_dfs_def wf_env_def unvisited_def)
+    next
+      case False
+      with \<open>x \<preceq> y in stack ?e'\<close> have "x \<preceq> y in stack e"
+        by (simp add: precedes_in_tail)
+      with asm assms show ?thesis
+        by (auto simp: pre_dfs_def wf_env_def unvisited_def)
+    qed
+  qed
+
+  ultimately have "wf_env ?e'" 
+    unfolding wf_env_def by blast
 
   moreover
-  have subsucc:"v \<in> visited ?e'" by simp
+  have "v \<in> visited ?e'"
+    by simp
+
+  moreover
+  from assms 
+  have "\<forall>w \<in> vsuccs ?e' v. w \<in> explored ?e' \<union> \<S> ?e' (hd (stack ?e'))"
+    by (simp add: pre_dfs_def)
 
   moreover
   have reachstack:"\<forall> n \<in> set (stack ?e'). reachable n v"
@@ -596,35 +655,27 @@ proof -
     by simp
 
   moreover
-  have "v \<in> \<S> ?e' (hd (stack ?e'))"
-    using "1"(5) by auto
-
-  moreover
   from \<open>pre_dfs v e\<close> have "\<S> ?e' (hd (stack ?e')) = {v}"
     by (simp add: pre_dfs_def wf_env_def)
 
   ultimately show ?thesis
-    unfolding pre_dfss_def by simp
+    unfolding pre_dfss_def by blast
 qed
 
 lemma pre_dfss_pre_dfs:
-  fixes w
-  assumes "pre_dfss v vs e" and "w \<notin> visited e" and "w \<in> vs"
+  assumes "pre_dfss v e" and "w \<notin> visited e" and "w \<in> successors v"
   shows "pre_dfs w e" 
-proof -
-  have "wf_env e"
-    using assms(1) pre_dfss_def by fastforce
-  thus ?thesis
-    by (meson assms(1) assms(2) assms(3) graph.pre_dfss_def graph_axioms in_mono pre_dfs_def succ_reachable) 
-qed
+  using assms unfolding pre_dfss_def pre_dfs_def wf_env_def
+  by (meson succ_reachable)
+
 
 lemma pre_dfs_implies_post_dfs:
   fixes v e
   defines "e1 \<equiv> e\<lparr>visited := visited e \<union> {v}, stack := (v # stack e)\<rparr>"
-  defines "e' \<equiv> dfss v (successors v) e1"
+  defines "e' \<equiv> dfss v e1"
   assumes 1: "pre_dfs v e"
       and 2: "dfs_dfss_dom (Inl(v, e))"
-      and 3: "post_dfss v (successors v) e1 e'"
+      and 3: "post_dfss v e1 e'"
   shows "post_dfs v e (dfs v e)"
 proof (cases "v = hd(stack e')")
   case True
@@ -637,106 +688,73 @@ proof (cases "v = hd(stack e')")
                             stack:=tl(stack e')\<rparr>" (is "_ = ?e2")
     unfolding e1_def e'_def
     using True assms(1) assms(2) dfs.psimps by force
+  from 3 have "wf_env e'"
+    by (simp add: post_dfss_def)
   have stack:"stack ?e2 = tl (stack e')" by simp
   have Se'e2_eq:"\<forall> x. \<S> e' x = \<S> ?e2 x"
     by simp
-  have sub:"sub_env e e1" unfolding sub_env_def
-    using e1_def by auto
-  have stacke1:"stack e' = stack e1"
+  have sub: "sub_env e e1"
+    by (auto simp: sub_env_def e1_def)
+  have stacke1: "stack e' = stack e1"
   proof -
-    obtain ns where ns_def:"stack e1 = ns @ (stack e')" using 3 unfolding post_dfss_def
-      by blast
+    obtain ns where ns_def:"stack e1 = ns @ (stack e')" 
+      using 3 unfolding post_dfss_def by blast
     have "ns = []"
     proof (rule ccontr)
       assume "ns \<noteq> []"
       hence "hd(ns) = v" using e1_def ns_def
-        by (metis hd_append2 list.sel(1) select_convs(5) surjective update_convs(5))
+        by (metis hd_append2 list.sel(1) select_convs(6) surjective update_convs(6))
       hence "\<not> distinct (stack e1)" using True ns_def \<open>ns \<noteq> []\<close>
         by (metis disjoint_iff_not_equal distinct_append hd_in_set notempty) 
-      then show False using e1_def
-        by (smt (verit, ccfv_threshold) "1" distinct.simps(2) in_mono pre_dfs_def select_convs(5) surjective update_convs(3) update_convs(5) wf_env_def)
+      with 1 e1_def show False
+        by (auto simp: pre_dfs_def wf_env_def)
     qed
     then show ?thesis using 3 True wf_env_def
       by (simp add: ns_def)
   qed
-  moreover have subenv:"sub_env e ?e2" 
+  from stacke1 have stack2: "stack ?e2 = stack e"
+    by (simp add: e1_def)
+
+  moreover have subenv: "sub_env e ?e2" 
   proof -
-    from 3 sub have e:"visited e \<subseteq> visited e'"
-      by (auto simp: post_dfss_def sub_env_def)
-    have e':"visited e' \<subseteq> visited ?e2" unfolding e'_def
-      by (simp add: dfs.psimps)
-    from e and e' have visited:"visited e \<subseteq> visited ?e2"
-      by blast
+    from sub 3 have "sub_env e e'"
+      unfolding post_dfss_def by (auto elim: sub_env_trans)
 
-    from 3 sub have e:"explored e \<subseteq> explored e'"
-      by (auto simp: post_dfss_def sub_env_def)
-    have e':"explored e' \<subseteq> explored ?e2" unfolding e'_def
-      by (simp add: dfs.psimps)
-    from e and e' have explored:"explored e \<subseteq> explored ?e2"
-      by blast
-
-    have S:"\<forall> v. \<S> e v \<subseteq> \<S> ?e2 v"
+    moreover
+    have "\<Union> {\<S> e n | n. n \<in> set (stack e)} \<subseteq> \<Union> {\<S> ?e2 n | n. n \<in> set (stack ?e2)}"
     proof -
-      from 3 sub have e:"\<forall> v. \<S> e v \<subseteq> \<S> e' v"
-        unfolding post_dfss_def sub_env_def by fast
-      have e':"\<forall> v. \<S> e' v \<subseteq> \<S> ?e2 v"
-        by (simp add: dfs.psimps)
-      from e and e' have "\<forall> v. \<S> e v \<subseteq> \<S> ?e2 v"
-        by blast
-      thus ?thesis by simp
+      from \<open>stack e' = stack e1\<close> have "stack ?e2 = stack e"
+        by (auto simp: e1_def)
+      with Se'e2_eq have "\<Union> {\<S> ?e2 n | n. n \<in> set (stack ?e2)} = \<Union> {\<S> e' n | n. n \<in> set (stack e)}"
+        by auto
+      with \<open>sub_env e e'\<close> show ?thesis
+        unfolding sub_env_def by fastforce
     qed
 
-    have union:"\<Union> {\<S> e n | n. n \<in> set (stack e)} \<subseteq> \<Union> {\<S> ?e2 n | n. n \<in> set (stack ?e2)}"
-    proof -
-      have "stack ?e2 = tl(stack e')"
-        using stack by blast
-      then have "... = stack e" using True
-        by (metis \<open>stack e' = v # tl (stack e')\<close> calculation e1_def list.inject select_convs(5) surjective update_convs(5))
-      hence incl:"\<Union> {\<S> ?e2 n | n. n \<in> set (stack ?e2)} = \<Union> {\<S> e' n | n. n \<in> set (stack e)}" using Se'e2_eq
-        by force
-      have "sub_env e1 e'"
-        using 3 post_dfss_def by auto
-      hence "sub_env e e'" using sub
-        by (meson order.trans sub_env_def)
-      {
-        fix n
-        assume "n \<in> \<Union> {\<S> e n | n. n \<in> set (stack e)}"
-        then obtain x where x_def:"n \<in> \<S> e x \<and> x \<in> set(stack e)"
-          by blast 
-        from \<open>sub_env e e'\<close> have "\<S> e x \<subseteq> \<S> e' x"
-          by (simp add: sub_env_def)
-        hence "n \<in> \<S> e' x"
-          using x_def by blast
-        hence "n \<in> \<Union> {\<S> e' n | n. n \<in> set (stack e)}"
-          using x_def by blast
-      }
-      then show ?thesis
-        using incl by fastforce
-    qed
-
-    from visited explored S union show ?thesis
-      using sub_env_def by blast
+    ultimately show ?thesis
+      by (auto simp: sub_env_def)
   qed
 
-  moreover have wfenv:"wf_env ?e2"
+  moreover have wfenv: "wf_env ?e2"
   proof -
     have "distinct (stack ?e2)"
-      using 3 by (auto simp: post_dfss_def wf_env_def distinct_tl)
+      using \<open>wf_env e'\<close> by (auto simp: wf_env_def distinct_tl)
   
     moreover have "set (stack ?e2) \<subseteq> visited ?e2"
     proof -
       have "set (stack ?e2) = set (tl (stack e'))" by simp
       also have "\<dots> \<subseteq> visited e'"
-        by (smt (verit, del_insts) "3" \<open>stack e' = v # tl (stack e')\<close> order_trans post_dfss_def set_subset_Cons wf_env_def)
+        by (smt (verit, del_insts) \<open>wf_env e'\<close> \<open>stack e' = v # tl (stack e')\<close> order_trans set_subset_Cons wf_env_def)
       finally show ?thesis by simp
     qed
   
     moreover have "explored ?e2 \<subseteq> visited ?e2"
     proof -
-      from 3 have "explored e' \<subseteq> visited e'"
-        unfolding post_dfss_def wf_env_def by simp
+      from \<open>wf_env e'\<close> have "explored e' \<subseteq> visited e'"
+        unfolding wf_env_def by simp
       moreover have "\<S> e' v \<subseteq> visited e'"
-        by (smt (verit, best) "3" graph.post_dfss_def graph_axioms notempty singletonD subsetD subsetI wf_env_def) 
+        using \<open>wf_env e'\<close>
+        by (smt (verit, best) notempty singletonD subsetD subsetI wf_env_def) 
       ultimately show ?thesis by simp
     qed
   
@@ -744,27 +762,28 @@ proof (cases "v = hd(stack e')")
     proof -
       {
         fix w
-        assume w1:"w\<in> explored ?e2" and w2:"w \<in> set(stack ?e2)"
-        have "explored ?e2 = explored e' \<union> \<S> e' v" "stack ?e2 = tl(stack e')" by auto
+        assume w1:"w \<in> explored ?e2" and w2:"w \<in> set(stack ?e2)"
+        have "explored ?e2 = explored e' \<union> \<S> e' v" "stack ?e2 = tl(stack e')" 
+          by auto
         have False
-        proof(cases "w\<in> explored e'")
+        proof(cases "w \<in> explored e'")
           case True
-          have "w \<in> explored e' \<inter> set(stack e')"
-            by (metis Int_iff \<open>stack ?e2 = tl (stack e')\<close> \<open>w \<in> explored e'\<close> empty_iff list.set_sel(2) notempty set_empty w2) 
-          thus ?thesis
-            by (smt (verit, ccfv_threshold) "3" emptyE post_dfss_def wf_env_def)
+          hence "w \<in> explored e' \<inter> set(stack e')"
+            by (metis Int_iff \<open>stack ?e2 = tl (stack e')\<close> empty_iff list.set_sel(2) notempty set_empty w2) 
+          with 3 show ?thesis
+            by (auto simp: post_dfss_def wf_env_def)
         next
           case False
-          have "w \<in> \<S> e' v"
-            using False w1 by auto 
-          have "w \<in> set(tl(stack e'))"
-            using w2 by force
-          hence "w \<noteq> v"
-            by (smt (verit, del_insts) "3" \<open>stack e' = v # tl (stack e')\<close> distinct.simps(2) graph.post_dfss_def graph_axioms wf_env_def)
-          hence "w \<in> \<S> e' w \<inter> \<S> e' v"
-            using "3" \<open>w \<in> \<S> e' v\<close> post_dfss_def wf_env_def by fastforce
-          thus ?thesis using 3 post_dfss_def wf_env_def
-            by (smt (verit) \<open>w \<in> set (tl (stack e'))\<close> \<open>w \<noteq> v\<close> empty_iff list.set_sel(2) notempty)
+          with w1 have "w \<in> \<S> e' v"
+            by auto 
+          from w2 have "w \<in> set(tl(stack e'))"
+            by simp
+          with 3 \<open>stack e' = v # tl (stack e')\<close> True have "w \<noteq> v"
+            by (auto simp: post_dfss_def wf_env_def)
+          with 3 \<open>w \<in> \<S> e' v\<close> \<open>w \<in> set (tl (stack e'))\<close> notempty
+          show ?thesis
+            unfolding post_dfss_def wf_env_def
+            by (metis (no_types, opaque_lifting) disjoint_iff list.set_sel(2))
         qed
       }
       hence "set (tl (stack e')) \<inter> \<S> e' v = {}" by auto
@@ -776,127 +795,57 @@ proof (cases "v = hd(stack e')")
       ultimately show ?thesis
         by (smt (verit, ccfv_threshold) Un_iff disjoint_iff empty_iff list.set(1) list.set_sel(2) notempty)
     qed
-  
-    moreover have "\<forall>v w. w \<in> \<S> ?e2 v \<longleftrightarrow> (\<S> ?e2 v = \<S> ?e2 w)"
-    proof -
-      have lr: "\<forall>v w. w \<in> \<S> ?e2 v \<longrightarrow> (\<S> ?e2 v = \<S> ?e2 w)"
-      proof (clarify)
-        fix v w
-        assume w: "w \<in> \<S> ?e2 v"
-        {
-          fix x
-          assume x_sev:"x \<in> \<S> ?e2 v"
-          have "x \<in> \<S> ?e2 w"
-          proof (cases "x\<in>\<S> e' w")
-            case True
-            hence "x\<in>\<S> e' v" using e'_def
-              using x_sev by fastforce 
-            then show ?thesis
-              by (simp add: True) 
-          next
-            case f:False
-            have False
-            proof (cases "x \<in> \<S> e' v")
-              case True
-              have "w \<in> \<S> e' v"
-                using w by auto
-              hence "\<S> e' v = \<S> e' w"
-                by (smt (verit, del_insts) "3" graph.post_dfss_def graph_axioms wf_env_def)
-             thus ?thesis
-                using True f by auto 
-            next
-              case False
-              have "\<S> e' v = \<S> ?e2 v" by simp
-              hence "x \<notin> \<S> ?e2 v"
-                using False by blast 
-              then show ?thesis
-                using x_sev by blast 
-            qed
-            thus ?thesis
-              by blast 
-          qed
-        }
-        moreover
-        {
-          fix x
-          assume x:"x \<in> \<S> ?e2 w"
-          have "x \<in> \<S> ?e2 v" 
-          proof (cases "w \<in> \<S> e' v")
-            case True
-            have "\<S> e' w = \<S> e' v"
-              by (smt (verit, del_insts) "3" True graph.post_dfss_def graph_axioms wf_env_def)
-            hence "\<S> ?e2 v = \<S> ?e2 w"
-              by simp
-            thus ?thesis using x by simp
-          next
-            case False
-            have False
-            proof -
-              from Se'e2_eq have "w \<notin> \<S> ?e2 v"
-                using False by blast
-              thus ?thesis
-                using w by blast 
-            qed
-            thus ?thesis
-              by blast 
-          qed
-        }
-        ultimately show "\<S> ?e2 v = \<S> ?e2 w"
-          by blast
+
+    moreover
+    from \<open>wf_env e'\<close> 
+    have "\<forall>v. vsuccs ?e2 v \<subseteq> successors v"
+         "\<forall>v. vsuccs ?e2 v \<subseteq> visited ?e2"
+         "\<forall>v. v \<notin> visited ?e2 \<longrightarrow> vsuccs ?e2 v = {}"
+      by (auto simp: wf_env_def)
+
+    moreover
+    {
+      fix u
+      assume "u \<in> explored ?e2"
+      have "vsuccs ?e2 u = successors u"
+      proof (cases "u \<in> explored e'")
+        case True
+        with \<open>wf_env e'\<close> show ?thesis
+          by (auto simp: wf_env_def)
+      next
+        case False
+        with \<open>u \<in> explored ?e2\<close> have "u \<in> \<S> e' v"
+          by simp
+(* idea: 
+   - if u=v then the assertion follows directly from post_dfss
+   - otherwise u must be in visited but no longer on the call stack,
+     and the successors of all these nodes have been explored
+*)
+        then show ?thesis
+          sorry
       qed
-      moreover have rl: "\<forall>v w. (\<S> ?e2 v = \<S> ?e2 w) \<longrightarrow> w \<in> \<S> ?e2 v"
-      proof (clarify)
-        fix v w
-        assume S: "\<S> ?e2 v = \<S> ?e2 w"
-        have "w \<in> \<S> ?e2 w"
-        proof (cases "w \<in> \<S> e w")
-          case True
-          with 3 show ?thesis
-            by (auto simp: post_dfss_def wf_env_def)
-        next
-          case False
-          with 1 show ?thesis
-            by (auto simp: pre_dfs_def wf_env_def)
-        qed
-        thus "w \<in> \<S> ?e2 v" using S
-          by blast
-      qed
-      from lr rl show ?thesis by blast
-    qed
-  
-    moreover have onStackOneRepr:"\<forall>v w. (v \<in> set (stack ?e2) \<and> w \<in> set (stack ?e2) \<and> v \<noteq> w) \<longrightarrow> (\<S> ?e2 v \<inter> \<S> ?e2 w = {})"
-    proof (clarify)
-      fix v w
-      assume asm: "v \<in> set (stack ?e2)" "w \<in> set (stack ?e2)" "v \<noteq> w"
-      from asm have v':"v \<in> set (stack e')"
-        by (metis empty_set insert_absorb insert_not_empty list.set_sel(2) notempty select_convs(5) surjective update_convs(5))
-      from asm have w':"w \<in> set (stack e')"
-        by (metis empty_set insert_absorb insert_not_empty list.set_sel(2) notempty select_convs(5) surjective update_convs(5))
-      from v' w' have "\<S> e' v \<inter> \<S> e' w = {}" using assms(5)
-        by (simp add: asm post_dfss_def wf_env_def)
-      then show "\<S> ?e2 v \<inter> \<S> ?e2 w = {}"
-        by simp
-    qed
-  
-    moreover have"(\<forall> v. v \<notin> visited ?e2 \<longrightarrow> \<S> ?e2 v = {v})"
-    proof (clarify)
-      fix v
-      assume "v \<notin> visited ?e2"
-      hence "v \<notin> visited e'"
-        by simp
-      hence 1:"\<S> e' v = {v}" using assms(5)
-        by (simp add: post_dfss_def wf_env_def)
-      from 1 Se'e2_eq show "\<S> ?e2 v = {v}" by blast
-    qed
-  
+    }
+
+    moreover
+    from \<open>wf_env e'\<close> have "\<forall>v w. w \<in> \<S> ?e2 v \<longleftrightarrow> (\<S> ?e2 v = \<S> ?e2 w)"
+      by (auto simp: wf_env_def)
+
+    moreover
+    from 3 Se'e2_eq stack
+    have onStackOneRepr: "\<forall>v w. (v \<in> set (stack ?e2) \<and> w \<in> set (stack ?e2) \<and> v \<noteq> w) \<longrightarrow> (\<S> ?e2 v \<inter> \<S> ?e2 w = {})"
+      unfolding post_dfss_def wf_env_def by (metis (no_types, lifting) list.set_sel(2))
+
+    moreover 
+    from \<open>wf_env e'\<close> have"(\<forall> v. v \<notin> visited ?e2 \<longrightarrow> \<S> ?e2 v = {v})"
+      by (auto simp: wf_env_def)
+
     moreover have "\<Union> {\<S> ?e2 v | v . v \<in> set (stack ?e2)} = visited ?e2 - explored ?e2"
     proof -
-      have 1:"\<Union> {\<S> e' v | v . v \<in> set (stack e')} = visited e' - explored e'" using assms(5)
-        by (simp add: post_dfss_def wf_env_def)
-      also have "... = \<Union> {\<S> ?e2 v | v . v \<in> set (stack e')}" using Se'e2_eq
-        using calculation by auto
-      have stack:"stack ?e2 = tl(stack e')" by simp
-      with True stack have stacke':"set (stack e') = set (stack ?e2)  \<union> {v}"
+      have 1: "\<Union> {\<S> e' v | v . v \<in> set (stack e')} = visited e' - explored e'"
+        using \<open>wf_env e'\<close> by (simp add: wf_env_def)
+      also have "\<dots> = \<Union> {\<S> ?e2 v | v . v \<in> set (stack e')}" 
+        using Se'e2_eq 1 by auto
+      with True stack have stacke':"set (stack e') = set (stack ?e2) \<union> {v}"
         by (metis Un_insert_right empty_iff empty_set list.exhaust_sel list.simps(15) notempty sup_bot.right_neutral)
       hence 2:"\<Union> {\<S> ?e2 v | v . v \<in> set (stack e')} = (\<Union>{\<S> ?e2 v | v . v \<in> set (stack ?e2)}) \<union> (\<S> ?e2 v)" by auto
       have exploredD:"explored e' = explored ?e2 - (\<S> ?e2 v)"
@@ -911,54 +860,57 @@ proof (cases "v = hd(stack e')")
         by simp
       hence "(\<Union>{\<S> ?e2 v | v . v \<in> set (stack ?e2)}) \<union> (\<S> ?e2 v) = visited ?e2 - (explored ?e2 - (\<S> ?e2 v))" using 1 2
         by simp
-      moreover have disjoint:"(\<Union>{\<S> ?e2 v | v . v \<in> set (stack ?e2)}) \<inter> (\<S> ?e2 v) = {}"
+      moreover 
+      have disjoint:"(\<Union>{\<S> ?e2 v | v . v \<in> set (stack ?e2)}) \<inter> (\<S> ?e2 v) = {}"
       proof -
-        have "\<forall> w. w \<in> set (stack ?e2) \<longrightarrow> \<S> ?e2 w \<inter> \<S> ?e2 v = {}" using onStackOneRepr
-          by (smt (verit, best) "3" Se'e2_eq True Un_empty Un_iff distinct.simps(2) graph.wf_env_def graph_axioms hd_Cons_tl insert_not_empty notempty post_dfss_def set_empty stack stacke')
+        from \<open>wf_env e'\<close> onStackOneRepr Se'e2_eq True notempty stack stacke'
+        have "\<forall> w. w \<in> set (stack ?e2) \<longrightarrow> \<S> ?e2 w \<inter> \<S> ?e2 v = {}" 
+          unfolding wf_env_def
+          by (smt (verit, best) Un_empty Un_iff distinct.simps(2) hd_Cons_tl insert_not_empty set_empty)
         thus ?thesis
           by blast
       qed
-      hence strong:"(\<Union>{\<S> ?e2 v | v . v \<in> set (stack ?e2)}) \<union> (\<S> ?e2 v) = (visited ?e2 - explored ?e2) \<union> (\<S> ?e2 v)"
-        using calculation(2) by auto
-      have magic:"(visited ?e2 - explored ?e2) \<inter> (\<S> ?e2 v) = {}" using 1 "2" exploredD
+      ultimately
+      have "(\<Union>{\<S> ?e2 v | v . v \<in> set (stack ?e2)}) \<union> (\<S> ?e2 v) = (visited ?e2 - explored ?e2) \<union> (\<S> ?e2 v)"
+        by auto
+      moreover
+      from 1 2 exploredD
+      have "(visited ?e2 - explored ?e2) \<inter> (\<S> ?e2 v) = {}" 
         by force
-      thus ?thesis using strong magic
+      ultimately show ?thesis
         by (smt (verit, best) Int_Un_distrib Int_commute Un_Int_eq(3) disjoint)
     qed
     
-    moreover have "\<forall> x y. x \<preceq> y in stack ?e2 \<longrightarrow> reachable y x"
-    proof (clarify)
-      fix x y
-      assume asm:"x \<preceq> y in stack ?e2"
-      with 3 have reachable:"\<forall> x y. x \<preceq> y in stack e' \<longrightarrow> reachable y x"
-        by (auto simp: post_dfss_def wf_env_def)
-      have "x \<preceq> y in stack e'" using stack asm
-        by (metis \<open>stack e' = v # tl (stack e')\<close> emptyE head_precedes list.set_sel(2) notempty precedes_in_tail precedes_mem(2) set_empty)
-      thus "reachable y x" using reachable by blast 
-    qed
-  
-    moreover have "\<forall> x. is_subscc (\<S> ?e2 x)" using assms(5)
-      by (simp add: post_dfss_def wf_env_def)
+    moreover
+    from 3 \<open>stack e' = v # tl (stack e')\<close> stack notempty
+    have "\<forall> x y. x \<preceq> y in stack ?e2 \<longrightarrow> reachable y x"
+      unfolding post_dfss_def wf_env_def
+      by (metis True precedes_in_tail precedes_mem(1))
 
-    moreover have "\<forall> x \<in> explored ?e2. \<forall> y. reachable x y \<longrightarrow> y \<in> explored ?e2"
+    moreover 
+    from \<open>wf_env e'\<close> have "\<forall> x. is_subscc (\<S> ?e2 x)"
+      by (simp add: wf_env_def)
+
+    moreover have "\<forall>x \<in> explored ?e2. \<forall>y. reachable x y \<longrightarrow> y \<in> explored ?e2"
     proof (clarify)
       fix x y
-      assume asm:"x \<in> explored ?e2" "reachable x y"
+      assume asm: "x \<in> explored ?e2" "reachable x y"
       show "y \<in> explored ?e2"
       proof (cases "x \<in> explored e'")
         case True
-        then show ?thesis using 3 wf_env_def unfolding wf_env_def
-          by (simp add: asm(2) post_dfss_def wf_env_def)
+        with \<open>wf_env e'\<close> \<open>reachable x y\<close> show ?thesis
+          by (simp add: wf_env_def)
       next
-        from notempty have stacke':"v \<in> set (stack e')"
-          by blast
         case False
         hence "x \<in> \<S> e' v" using asm
           by simp
-        hence "reachable v y" using asm(2) assms(5)
-          by (metis Se'e2_eq calculation(10) calculation(5) is_subscc_def reachable_trans)
-        hence visitedy:"y \<in> visited e'" using assms(5) stacke' unfolding post_dfss_def
-          by (smt (verit, best) in_mono reachable.cases wf_env_def)
+        with \<open>wf_env e'\<close> have "reachable v x"
+          by (auto simp: wf_env_def is_subscc_def)
+        from this \<open>reachable x y\<close> have "reachable v y"
+          by (rule reachable_trans)
+        with 3 \<open>v = hd (stack e')\<close>
+        have visitedy: "y \<in> visited e'"
+          by (auto simp: post_dfss_def)
         show ?thesis
         proof (cases "y \<in> explored e'")
           case True
@@ -966,9 +918,9 @@ proof (cases "v = hd(stack e')")
             by simp
         next
           case False
-          from False visitedy have "y \<in> \<Union> {\<S> e' v | v. v \<in> set (stack e')}" using wf_env_def[of e'] assms(5)
-            by (simp add: post_dfss_def)
-          then obtain n where ndef: "n \<in> set (stack e') \<and> (y \<in> \<S> e' n)"
+          from False visitedy \<open>wf_env e'\<close> have "y \<in> \<Union> {\<S> e' v | v. v \<in> set (stack e')}"
+            by (simp add: wf_env_def)
+          then obtain n where ndef: "n \<in> set (stack e')" "(y \<in> \<S> e' n)"
             by force
           show ?thesis
           proof (cases "n = v")
@@ -980,8 +932,8 @@ proof (cases "v = hd(stack e')")
             have "n \<in> set (tl (stack e'))"
               by (metis set_ConsD)
             moreover
-            from 3 have "is_subscc (\<S> e' n)" "n \<in> \<S> e' n"
-              unfolding post_dfss_def wf_env_def by auto
+            from \<open>wf_env e'\<close> have "is_subscc (\<S> e' n)" "n \<in> \<S> e' n"
+              unfolding wf_env_def by auto
             with ndef have "reachable y n"
               by (auto simp: is_subscc_def)
             hence "reachable v n"
@@ -1000,85 +952,87 @@ proof (cases "v = hd(stack e')")
       show "is_scc S"
       proof (cases "S = \<S> e' v")
         case True
-        hence nemp:"S \<noteq> {}"
-          using Se'e2_eq calculation(5) by blast
-        have subscc:"is_subscc S"
-          using True calculation(10) by fastforce
+        with \<open>wf_env e'\<close> have "S \<noteq> {}"
+          unfolding wf_env_def by (metis empty_iff)
+        from \<open>wf_env e'\<close> True have subscc:"is_subscc S"
+          by (simp add: wf_env_def)
         {
-          assume contrad:"\<not> is_scc S"
-          then obtain S' where S'_def:"S' \<noteq> S \<and> S \<subseteq> S' \<and> is_subscc S'" unfolding is_scc_def
-            using nemp subscc by blast
+          assume contrad: "\<not> is_scc S"
+          with \<open>S \<noteq> {}\<close> \<open>is_subscc S\<close> obtain S' where
+            S'_def: "S' \<noteq> S" "S \<subseteq> S'" "is_subscc S'" 
+            unfolding is_scc_def by blast
           then obtain x where "x \<in> S' \<and> x \<notin> S"
             by blast
-          hence xv:"reachable v x \<and> reachable x v"
-            by (metis Se'e2_eq True S'_def calculation(5) in_mono is_subscc_def)
-          have "\<S> e' v =  \<S> e' x"
-          proof (cases "x \<in> set (stack e')")
-            case True
-            with 3 xv \<open>stack e' = v # tl(stack e')\<close> show ?thesis
-              by (smt (verit) list.sel(1) post_dfss_def set_ConsD)
-          next
-            case False
-            have "x \<in> explored e'"
-              using True \<open>x \<in> S' \<and> x \<notin> S\<close> calculation(11) calculation(5) xv by auto
-            from assms(5) have "\<forall> x \<in> explored e'. \<forall> y. reachable x y \<longrightarrow> y \<in> explored e'" using post_dfss_def unfolding wf_env_def
-              by (simp add: post_dfss_def wf_env_def)
-            hence "v \<in> explored e'" using False
-              using \<open>x \<in> explored e'\<close> xv by blast
-            with 3 notempty show ?thesis
-              unfolding post_dfss_def wf_env_def by auto
-          qed
-          then have "is_scc S"
-            using Se'e2_eq True \<open>x \<in> S' \<and> x \<notin> S\<close> calculation(5) by blast
+          with True S'_def \<open>wf_env e'\<close>
+          have xv: "reachable v x \<and> reachable x v"
+            unfolding wf_env_def is_subscc_def by (metis in_mono)
+          from \<open>\<forall>v w. w \<in> \<S> ?e2 v \<longleftrightarrow> (\<S> ?e2 v = \<S> ?e2 w)\<close>
+          have "v \<in> explored ?e2"
+            by auto
+          with \<open>\<forall> x \<in> explored ?e2. \<forall> y. reachable x y \<longrightarrow> y \<in> explored ?e2\<close>
+               xv \<open>S = \<S> e' v\<close> \<open>x \<in> S' \<and> x \<notin> S\<close>
+          have "x \<in> explored e'"
+            by auto
+          with \<open>wf_env e'\<close> xv have "v \<in> explored e'"
+            by (auto simp: wf_env_def)
+          with \<open>wf_env e'\<close> notempty have "\<S> e' v =  \<S> e' x"
+            by (auto simp: wf_env_def)
+          with \<open>wf_env e'\<close> have "x \<in> \<S> e' v"
+            by (auto simp: wf_env_def)
+          with \<open>S = \<S> e' v\<close> \<open>x \<in> S' \<and> x \<notin> S\<close> have "False"
+            by simp
         }
         then show ?thesis
           by blast
       next
         case False
-        with asm 3 show ?thesis
-          by (auto simp: post_dfss_def wf_env_def)
+        with asm \<open>wf_env e'\<close> show ?thesis
+          by (auto simp: wf_env_def)
       qed
     qed
-    
+
+    moreover
+    {
+      fix x y u
+      assume xy: "x \<preceq> y in stack ?e2" "x \<noteq> y"
+         and u: "u \<in> \<S> ?e2 x" "reachable_avoiding u y (unvisited ?e2 x)"
+      from xy \<open>stack e' = v # (tl (stack e'))\<close>
+      have "x \<preceq> y in stack e'"
+        by (metis head_precedes list.set_intros(2) precedes_in_tail precedes_mem(2) stack)
+      with \<open>wf_env e'\<close> \<open>x \<noteq> y\<close> u have "False"
+        by (auto simp: wf_env_def unvisited_def)
+    }
+
     ultimately show ?thesis unfolding wf_env_def
       by meson
   qed
 
-  moreover have reachable_visited:"\<forall> x. reachable v x \<longrightarrow> x \<in> visited ?e2"
-  proof (clarify)
-    fix x
-    assume "reachable v x"
-    then show "x \<in> visited ?e2" using 3 post_dfss_def reachable.cases notempty wf_env_def
-      by (smt (verit, best) ext_inject subset_iff surjective update_convs(2) update_convs(4) update_convs(5))
-  qed
-
-  moreover have stack_reachable:"\<forall> n \<in> set (stack ?e2). reachable n v" 
-    using assms stack unfolding post_dfss_def
-    by (metis list.set_sel(2))
-
-  moreover have "\<exists> ns. stack e = ns @ (stack ?e2)"
-  proof -
-    have "stack ?e2 = tl(stack e')"
-      using stack by blast
-    then have "... = stack e" using True
-      by (metis \<open>stack e' = v # tl (stack e')\<close> calculation(1) e1_def list.inject select_convs(5) surjective update_convs(5))
-    thus ?thesis
-      by simp
-  qed
-
-
-  moreover have stack:"stack ?e2 = tl(stack e')" by simp
-  with True stack have stacke':"set (stack e') = set (stack ?e2)  \<union> {v}"
-    by (metis Un_insert_right empty_iff empty_set list.exhaust_sel list.simps(15) notempty sup_bot.right_neutral)
-
   moreover 
-  from stacke1 stack stacke' have "stack ?e2 = stack e"
-    by (auto simp: e1_def)
+  from \<open>wf_env ?e2\<close> have "v \<in> explored ?e2"
+    by (auto simp: wf_env_def)
 
   moreover
-  from 3 True have "v \<in> explored ?e2"
-    by (auto simp: post_dfss_def)
-  
+  from \<open>v \<in> explored ?e2\<close> \<open>wf_env ?e2\<close>
+  have reachable_visited:"\<forall> x. reachable v x \<longrightarrow> x \<in> visited ?e2"
+    unfolding wf_env_def by (meson in_mono)
+
+  moreover
+  from 3 have "vsuccs ?e2 v = successors v"
+    by (simp add: post_dfss_def)
+
+  moreover
+  from 1 3 have "\<forall>w \<in> visited e. vsuccs ?e2 w = vsuccs e w"
+    by (auto simp: pre_dfs_def post_dfss_def e1_def)
+
+  moreover 
+  from stack2 1 
+  have stack_reachable: "\<forall>n \<in> set (stack ?e2). reachable n v"
+    by (simp add: pre_dfs_def)
+
+  moreover 
+  from stack2 have "\<exists> ns. stack e = ns @ (stack ?e2)"
+    by auto
+
   moreover
   from 3 have "\<forall>n \<in> set (stack ?e2). \<S> ?e2 n = \<S> e n"
     by (auto simp: post_dfss_def e1_def)
@@ -1090,59 +1044,45 @@ next
   with 2 have e':"dfs v e = e'"
     unfolding e1_def e'_def by (simp add: dfs.psimps)
 
-  moreover from 3 have wfenv:"wf_env e'" 
+  moreover from 3 have wfenv: "wf_env e'" 
     by (simp add: post_dfss_def)
+
+  moreover from 3 have "v \<in> visited e'"
+    by (auto simp: post_dfss_def sub_env_def e1_def)
 
   moreover have subenv:"sub_env e e'"
   proof -
     have "sub_env e e1"
-      unfolding sub_env_def
-      by (auto simp: e1_def)
+      unfolding sub_env_def by (auto simp: e1_def)
     with 3 show ?thesis
-      unfolding post_dfss_def sub_env_def 
-      by (meson subset_trans)
+      unfolding post_dfss_def by (auto elim: sub_env_trans)
   qed
 
-  moreover have reachable_visited:"(\<forall> x. reachable v x \<longrightarrow> x \<in> visited e')"
-  proof (clarify)
-    fix x
-    assume asm:"reachable v x"
-    show "x \<in> visited e'"
-    proof (cases "x = v")
-      case True
-      have "visited e1 \<subseteq> visited e'"
-        using 3 dfs.psimps dfss.psimps
-        unfolding post_dfss_def
-        by (metis sub_env_def)
-      have v:"v \<in> visited e1"
-        by (simp add: e1_def)
-      thus ?thesis
-        using True \<open>visited e1 \<subseteq> visited e'\<close> by auto
-    next
-      case False
-      obtain w where "w \<in> (successors v) \<and> reachable w x" using False
-        by (meson asm reachable.cases)
-      with 3 show ?thesis
-        by (auto simp: post_dfss_def)
-    qed
-  
-  qed
+  moreover
+  from 3 have "vsuccs e' v = successors v"
+    by (simp add: post_dfss_def)
+
+  moreover
+  from 1 3 have "\<forall>w \<in> visited e. vsuccs e' w = vsuccs e w"
+    by (auto simp: pre_dfs_def post_dfss_def e1_def)
+
+  moreover 
+  from 3
+  have reachable_visited: 
+    "(\<forall>x. reachable v x \<longrightarrow> x \<in> visited e' \<or> (\<exists>n \<in> set (tl (stack e')). reachable v n \<and> reachable n x))"
+    by (auto simp: post_dfss_def)
 
   moreover have stack_visited: "\<forall> n \<in> set (stack e'). reachable n v"
     using 3 by (auto simp: post_dfss_def)
 
   moreover have "\<exists> ns. stack e = ns @ (stack e')"
   proof -
-    from 3 obtain ns where "stack e1 = ns @ stack e'"
+    from 3 obtain ns where ns: "stack e1 = ns @ stack e'"
       unfolding post_dfss_def by blast
-    moreover have "... = v # stack e" using e1_def
-      using calculation by simp
-    moreover have "ns \<noteq> []" using False
-      using calculation by auto
-    moreover have "stack e = tl(ns) @ stack e'"
-      by (metis calculation(2) calculation(3) list.sel(3) tl_append2)
-    ultimately show ?thesis
-      by blast
+    with False have "stack e = (tl ns) @ stack e'"
+      unfolding e1_def
+      by (metis list.sel(1) list.sel(3) select_convs(6) self_append_conv2 surjective tl_append2 update_convs(6))
+    thus ?thesis by blast
   qed
 
   moreover
@@ -1150,48 +1090,6 @@ next
        "\<forall>n \<in> set (tl (stack e')). \<S> e' n = \<S> e n"
     using 3 by (auto simp: post_dfss_def e1_def)
 
-  moreover
-  have "(\<forall>n \<in> set (tl (stack e')). \<forall>w \<in> \<S> e' (hd (stack e')) - \<S> e (hd (stack e')).
-               \<not> reachable_avoiding w n (\<S> e' (hd (stack e'))))"
-    sorry
-(*
-  proof (clarify)
-    fix n w
-    assume asm: "v = hd (stack e')" 
-                "n \<in> set (tl (stack e'))" "w \<in> \<S> e' (hd (stack e'))"
-                "reachable_avoiding w n (\<S> e' (hd (stack e')))"
-    show "False"
-    proof (cases "w = v")
-      case True
-      with \<open>stack e' \<noteq> []\<close> \<open>v \<in> \<S> e' (hd (stack e'))\<close> 
-           \<open>n \<in> set (tl (stack e'))\<close> \<open>wf_env e'\<close>
-      have "v \<noteq> n" 
-        unfolding wf_env_def
-        by (metis (no_types, lifting) Diff_cancel Diff_triv False empty_iff list.set_sel)
-      with True asm obtain w' where
-        w': "w' \<in> successors v - {v}" "reachable_avoiding w' n (\<S> e' (hd (stack e')))"
-        using ra_cases by blast
-      show ?thesis
-      proof (cases "w' \<in> explored e'")
-        case True
-        with ra_reachable[OF \<open>reachable_avoiding w' n (\<S> e' (hd (stack e')))\<close>]
-             \<open>stack e' \<noteq> []\<close> \<open>n \<in> set (tl (stack e'))\<close> \<open>wf_env e'\<close>
-        show ?thesis unfolding wf_env_def by (meson disjoint_iff list.set_sel(2))
-      next
-        case False
-        with 3 \<open>v = hd (stack e')\<close> 
-             \<open>w' \<in> successors v - {v}\<close> \<open>n \<in> set (tl (stack e'))\<close>
-             \<open>reachable_avoiding w' n (\<S> e' (hd (stack e')))\<close>
-        show ?thesis
-          by (auto simp: post_dfss_def)
-      qed
-    next
-      case False
-      with 3 asm show ?thesis 
-        by (auto simp: post_dfss_def)
-    qed
-  qed
-*)
   ultimately show ?thesis unfolding post_dfs_def
     by blast
 qed
@@ -1199,265 +1097,208 @@ qed
 lemma partial_correctness:
   shows
   "\<lbrakk>dfs_dfss_dom (Inl(v,e)); pre_dfs v e\<rbrakk> \<Longrightarrow> post_dfs v e (dfs v e)"
-  "\<lbrakk>dfs_dfss_dom (Inr(v,vs,e)); pre_dfss v vs e\<rbrakk> \<Longrightarrow> post_dfss v vs e (dfss v vs e)"
+  "\<lbrakk>dfs_dfss_dom (Inr(v,e)); pre_dfss v e\<rbrakk> \<Longrightarrow> post_dfss v e (dfss v e)"
 proof (induct rule: dfs_dfss.pinduct)
   fix v e
-  assume dom:"dfs_dfss_dom (Inl(v,e))"
-     and predfs:"pre_dfs v e"
-     and prepostdfss:"\<And>e1. \<lbrakk> e1 = e \<lparr>visited := visited e \<union> {v}, stack := v # stack e\<rparr>; pre_dfss v (successors v) e1 \<rbrakk>
-               \<Longrightarrow> post_dfss v (successors v) e1 (dfss v (successors v) e1)"
+  assume dom: "dfs_dfss_dom (Inl(v,e))"
+     and predfs: "pre_dfs v e"
+     and prepostdfss: "\<And>e1. \<lbrakk> e1 = e \<lparr>visited := visited e \<union> {v}, stack := v # stack e\<rparr>; pre_dfss v e1 \<rbrakk>
+                            \<Longrightarrow> post_dfss v e1 (dfss v e1)"
   then show "post_dfs v e (dfs v e)"
     using pre_dfs_implies_post_dfs pre_dfs_pre_dfss by auto
 next
-  fix v vs e
-  assume dom:"dfs_dfss_dom (Inr(v,vs,e))"
-     and predfss:"pre_dfss v vs e"
-     and prepostdfs:"\<And>w. \<lbrakk> vs \<noteq> {}; w = (SOME x. x \<in> vs); w \<notin> explored e; w \<notin> visited e; pre_dfs w e \<rbrakk> \<Longrightarrow> post_dfs w e (dfs w e)"
-     and prepostdfss:"\<And>w e'. \<lbrakk> vs \<noteq> {}; w = (SOME x. x \<in> vs); e' = (if w \<in> explored e then e else if w \<notin> visited e then dfs w e else unite v w e);pre_dfss v (vs - {w}) e' \<rbrakk> \<Longrightarrow> post_dfss v (vs - {w}) e' (dfss v (vs - {w}) e')"
-  show "post_dfss v vs e (dfss v vs e)"
-  proof (cases "vs = {}")
-    case True
-    hence return_e:"dfss v vs e = e" using dom dfss.psimps by metis
-    moreover have "wf_env e"
-      using predfss by (simp add: pre_dfss_def)
-    moreover have "\<forall>w \<in> vs. \<forall>x. reachable w x \<longrightarrow> x \<in> visited e"
-      by (simp add: True)
-    moreover have "sub_env e e"
-      by (simp add: sub_env_def)
-    moreover have "\<forall>w \<in> successors v. w \<in> explored e \<union> \<S> e (hd (stack e))"
-      using predfss True by (simp add: pre_dfss_def)
-    moreover have "\<forall> n \<in> set (stack e). reachable n v"
-      using pre_dfss_def predfss by blast
-    moreover have "stack e \<noteq> []"
-      using pre_dfss_def predfss by blast
-    moreover have "\<exists> ns. stack e = ns @ (stack e)"
-      by simp
-    moreover have "v \<in> \<S> e (hd (stack e))"
-      using pre_dfss_def predfss by blast
-    moreover
-    have "hd (stack e) = v \<longrightarrow>
-             (\<forall>n \<in> set (tl (stack e)). \<forall>w \<in> \<S> e (hd (stack e)) - {v}.
-                 \<not> reachable_avoiding w n (\<S> e (hd (stack e))))"
-      using predfss by (auto simp: pre_dfss_def)
-    moreover
-    {
-      fix n
-      assume asm: "hd (stack e) = v"
-                  "n \<in> set (tl (stack e))"
-                  "reachable v n"
-      from \<open>v \<in> \<S> e (hd (stack e))\<close> \<open>reachable v n\<close>
-      obtain w where "w \<in> \<S> e (hd (stack e))" "reachable_avoiding w n (\<S> e (hd (stack e)))"
-        using reach_avoid by blast
-      with predfss \<open>hd (stack e) = v\<close> \<open>n \<in> set (tl (stack e))\<close> have "w = v"
-        by (auto simp: pre_dfss_def)
-      from asm \<open>stack e \<noteq> []\<close> \<open>wf_env e\<close> have "v \<noteq> n"
-        unfolding wf_env_def by (metis distinct.simps(2) hd_Cons_tl)
-      with ra_cases[OF \<open>reachable_avoiding w n (\<S> e (hd (stack e)))\<close>] \<open>w = v\<close> 
-      obtain w' where
-        w': "w' \<in> successors v" "w' \<notin> \<S> e (hd (stack e))"
-            "reachable_avoiding w' n (\<S> e (hd (stack e)))"
-        by blast
-      with predfss \<open>vs = {}\<close> have "w' \<in> explored e"
-        by (auto simp: pre_dfss_def)
-      with ra_reachable[OF \<open>reachable_avoiding w' n (\<S> e (hd (stack e)))\<close>]
-           \<open>n \<in> set (tl (stack e))\<close> \<open>stack e \<noteq> []\<close> \<open>wf_env e\<close>
-      have "False"
-        unfolding wf_env_def by (metis Int_iff empty_iff list.set_sel(2))
-    }
-    ultimately show ?thesis
-      by (force simp: post_dfss_def)
-  next
-    case vs_case: False
-    define w where "w = (SOME x. x \<in> vs)"
-    define e' where "e' = (if w \<in> explored e then e else if w \<notin> visited e then dfs w e else unite v w e)"
-    from vs_case have wvs: "w \<in> vs"
-      unfolding w_def by (simp add: some_in_eq)
+  fix v e
+  assume dom: "dfs_dfss_dom (Inr(v,e))"
+     and predfss: "pre_dfss v e"
+     and prepostdfs: 
+           "\<And>vs w. 
+             \<lbrakk> vs = successors v - vsuccs e v; vs \<noteq> {}; w = (SOME x. x \<in> vs); 
+               w \<notin> explored e; w \<notin> visited e; pre_dfs w e \<rbrakk>
+             \<Longrightarrow> post_dfs w e (dfs w e)"
+     and prepostdfss:
+           "\<And>vs w e' e''. 
+             \<lbrakk> vs = successors v - vsuccs e v; vs \<noteq> {}; w = (SOME x. x \<in> vs); 
+               e' = (if w \<in> explored e then e 
+                     else if w \<notin> visited e then dfs w e 
+                     else unite v w e); 
+               e'' = e'\<lparr>vsuccs := \<lambda>x. if x = v then vsuccs e' v \<union> {w} 
+                                      else vsuccs e' x\<rparr> ;
+               pre_dfss v e'' \<rbrakk>
+             \<Longrightarrow> post_dfss v e'' (dfss v e'')"
+  show "post_dfss v e (dfss v e)"
+  proof -
+    let ?vs = "successors v - vsuccs e v"
+    from predfss have "v \<in> visited e"
+      by (simp add: pre_dfss_def)
+    from predfss have "v \<notin> explored e"
+      unfolding pre_dfss_def wf_env_def is_subscc_def
+      by (metis disjoint_iff list.set_sel(1))
+
     show ?thesis
-    proof (cases "w \<in> explored e")
+    proof (cases "?vs = {}") 
       case True
-      hence dfss: "dfss v vs e = dfss v (vs - {w}) e'"
-        by (simp add: dom vs_case w_def dfss.psimps e'_def)
-
-      from True have env_eq: "e' = e" by (simp add: e'_def)
-(*
-      with predfss True have "pre_dfss v (vs - {w}) e'"
-        by (auto simp: pre_dfss_def wf_env_def) -- works, very slow 
-*)
-      have "pre_dfss v (vs - {w}) e'"
-      proof -
-        from predfss env_eq have "pre_dfss v vs e'"
-          by simp
-        hence "wf_env e'" 
-              "v \<in> visited e'" 
-              "vs - {w} \<subseteq> successors v"
-              "\<forall>n \<in> set (stack e'). reachable n v"
-              "stack e' \<noteq> []"
-              "v \<in> \<S> e' (hd (stack e'))"
-              "hd (stack e') = v \<longrightarrow>
-                  (\<forall>n \<in> set (tl (stack e')). \<forall>w \<in> \<S> e' (hd (stack e')) - {v}.
-                      \<not> reachable_avoiding w n (\<S> e' (hd (stack e'))))"
-          by (auto simp: pre_dfss_def)
+      with dom have return_e: "dfss v e = e" 
+        by (simp add: dfss.psimps)
+      moreover have "wf_env e"
+        using predfss by (simp add: pre_dfss_def)
+      moreover have "vsuccs e v = successors v"
+        using True \<open>wf_env e\<close> unfolding wf_env_def
+        by (meson Diff_eq_empty_iff subset_antisym)
+      moreover
+      {
+        fix x
+        assume x: "reachable v x"
+        have "x \<in> visited e \<or> (\<exists>n \<in> set (tl (stack e)). reachable v n \<and> reachable n x)"
+          sorry
+      }
+      moreover have "sub_env e e"
+        by (simp add: sub_env_def)
+      moreover have "\<forall>w \<in> successors v. w \<in> explored e \<union> \<S> e (hd (stack e))"
+        using predfss \<open>vsuccs e v = successors v\<close> by (simp add: pre_dfss_def)
+      moreover have "\<forall> n \<in> set (stack e). reachable n v"
+        using pre_dfss_def predfss by blast
+      moreover have "stack e \<noteq> []"
+        using pre_dfss_def predfss by blast
+      moreover have "\<exists> ns. stack e = ns @ (stack e)"
+        by simp
+      moreover have "v \<in> \<S> e (hd (stack e))"
+        using pre_dfss_def predfss by blast
+      moreover
+      {
+        fix n
+        assume asm: "hd (stack e) = v"
+                    "n \<in> set (tl (stack e))"
+                    "reachable v n"
+        with \<open>stack e \<noteq> []\<close> have "v \<preceq> n in stack e"
+          by (metis head_precedes hd_Cons_tl list.set_sel(2))
         moreover
-        {
-          fix u
-          assume u: "u \<in> successors v - (vs - {w})"
-          have "u \<in> explored e' \<union> \<S> e' (hd (stack e'))"
-          proof (cases "u = w")
-            case True
-            with \<open>w \<in> explored e\<close> show ?thesis
-              by (simp add: env_eq)
-          next
-            case False
-            with u predfss show ?thesis
-              by (simp add: pre_dfss_def env_eq)
-          qed
-        }
-        ultimately show ?thesis
-          by (auto simp: pre_dfss_def)
-      qed
-
-      then have post: "post_dfss v (vs - {w}) e' (dfss v (vs - {w}) e')"
-        using True \<open>e' = e\<close> prepostdfss vs_case w_def by auto
-
-      moreover have wfenv: "wf_env (dfss v vs e)"
-        using dfss post by (auto simp: post_dfss_def)
-      moreover have reach:"\<forall> u \<in> vs. \<forall> x. reachable u x \<longrightarrow> x \<in> visited (dfss v vs e)"
-      proof (clarify)
-        fix u x
-        assume asm:"u \<in> vs" "reachable u x"
-        show "x \<in> visited (dfss v vs e)"
-        proof (cases "u = w")
-          case True
-          with \<open>w \<in> explored e\<close> \<open>e' = e\<close> asm wfenv dfss post
-          show ?thesis unfolding wf_env_def post_dfss_def sub_env_def
-            by (metis subset_eq)
-        next
-          case False
-          with asm post dfss \<open>e' = e\<close> show ?thesis
-            by (auto simp: post_dfss_def)
-        qed
-      qed
-
+        from \<open>wf_env e\<close> \<open>stack e \<noteq> []\<close> asm have "v \<noteq> n"
+          unfolding wf_env_def
+          by (metis distinct.simps(2) list.exhaust_sel)
+        moreover
+        from \<open>wf_env e\<close> have "v \<in> \<S> e v"
+          by (auto simp: wf_env_def)
+        moreover
+        have "unvisited e v = {}"
+        (* proof analogous to the sketch above *)
+          sorry
+        ultimately have "\<not> reachable_avoiding v n {}"
+          using \<open>wf_env e\<close> unfolding wf_env_def by metis
+        with \<open>reachable v n\<close> have "False"
+          by (simp add: ra_empty)
+      }
       ultimately show ?thesis
-        by (simp add: env_eq dfss post_dfss_def)
+        by (force simp: post_dfss_def)
     next
-      case notexplored: False
-      then show ?thesis
-      proof (cases "w \<notin> visited e")
+      case vs_case: False
+      define w where "w = (SOME x. x \<in> ?vs)"
+      define e' where "e' = (if w \<in> explored e then e 
+                             else if w \<notin> visited e then dfs w e 
+                             else unite v w e)"
+      define e'' where "e'' = (e'\<lparr>vsuccs := \<lambda>x. if x=v then vsuccs e' v \<union> {w} else vsuccs e' x\<rparr>)"
+
+      from dom vs_case have dfss: "dfss v e = dfss v e''"
+        apply (auto simp: dfss.psimps w_def e'_def e''_def)
+        using w_def e'_def by auto
+
+      from vs_case have wvs: "w \<in> ?vs"
+        unfolding w_def by (metis some_in_eq)
+      show ?thesis
+      proof (cases "w \<in> explored e")
         case True
-        hence "e' = dfs w e" using e'_def notexplored
-          by auto
-        hence postdfsw: "post_dfs w e e'"
-          using True notexplored pre_dfss_pre_dfs predfss prepostdfs some_in_eq vs_case w_def by blast
-        moreover have "dfss v vs e = dfss v (vs - {w}) e'"
-          using True dfss.psimps dom e'_def notexplored vs_case w_def by force
-        moreover have "pre_dfss v (vs - {w}) e'"
+        hence e': "e' = e"
+          by (simp add: e'_def)
+
+        have "wf_env e''"
         proof -
-          from postdfsw have "wf_env e'"
-            using post_dfs_def by blast
-          moreover have "v \<in> visited e'"
-            by (metis graph.post_dfs_def graph_axioms in_mono postdfsw pre_dfss_def predfss sub_env_def)
-          moreover have "vs - {w} \<subseteq> successors v"
-            by (metis Diff_subset pre_dfss_def predfss subset_trans)
-          
-          moreover have "\<forall> n \<in> set (stack e'). reachable n v" 
-            using postdfsw post_dfs_def
-            by (metis Un_iff pre_dfss_def predfss set_append)
-
-          moreover have "stack e' \<noteq> []"
-          proof -
-            have "v \<notin> explored e"
-            proof (rule ccontr)
-              assume contrad:"\<not> v \<notin> explored e"
-              have "w \<in> vs" using w_def
-                using some_in_eq vs_case by blast
-              then show False using notexplored wf_env_def predfss pre_dfss_def contrad
-                by (smt (verit, best) in_mono reachable_edge)
-            qed
-
-            moreover have "v \<in> visited e"
-              using pre_dfss_def predfss by blast
-            
-            ultimately show ?thesis
-            proof -
-              have "v \<in> visited e - explored e"
-                by (simp add: \<open>v \<in> visited e\<close> \<open>v \<notin> explored e\<close>)
-              hence "v \<in> \<Union> {\<S> e v | v. v \<in> set (stack e)}" using predfss wf_env_def unfolding wf_env_def
-                by (simp add: pre_dfss_def wf_env_def)
-              then obtain u where u_def:"u \<in> set (stack e)" "v \<in> \<S> e u" using pre_dfss_def predfss wf_env_def 
-                by blast
-              from predfss have "u \<in> \<S> e u"
-                by (auto simp: pre_dfss_def wf_env_def)
-              hence "u \<in> \<Union>{\<S> e n | n. n \<in> set (stack e)}" using u_def(1)
-                by blast
-              moreover have "sub_env e e'"
-                using post_dfs_def postdfsw by blast
-              hence "u \<in> \<Union>{\<S> e' n | n. n \<in> set (stack e')}" using calculation unfolding sub_env_def
-                by blast
-              thus ?thesis
-                by force
-            qed
-          qed
-
-          moreover have "\<exists> ns. stack e = ns @ (stack e')"
-            using post_dfs_def postdfsw by blast
-
+          from predfss e' have wf': "wf_env e'"
+            by (simp add: pre_dfss_def)
+          hence "distinct (stack e'')"
+                "set (stack e'') \<subseteq> visited e''"
+                "explored e'' \<subseteq> visited e''"
+                "explored e'' \<inter> set (stack e'') = {}"
+                "\<forall>v w. w \<in> \<S> e'' v \<longleftrightarrow> (\<S> e'' v = \<S> e'' w)"
+                "\<forall>v \<in> set (stack e''). \<forall> w \<in> set (stack e''). 
+                    v \<noteq> w \<longrightarrow> \<S> e'' v \<inter> \<S> e'' w = {}"
+                "\<forall> v. v \<notin> visited e'' \<longrightarrow> \<S> e'' v = {v}"
+                "\<Union> {\<S> e'' v | v. v \<in> set (stack e'')} = visited e'' - explored e''"
+                "\<forall>x y. x \<preceq> y in stack e'' \<longrightarrow> reachable y x"
+                "\<forall>x. is_subscc (\<S> e'' x)"
+                "\<forall> x \<in> explored e''. \<forall> y. reachable x y \<longrightarrow> y \<in> explored e''"
+                "\<forall> S \<in> sccs e''. is_scc S"
+            by (auto simp: wf_env_def e''_def)
           moreover
-          {
-            fix u
-            assume u: "u \<in> successors v - (vs - {w})"
-            have "u \<in> explored e' \<union> \<S> e' (hd (stack e'))"
-            proof (cases "u = w")
-              case True
-              with postdfsw show ?thesis
-                by (auto simp: post_dfs_def)
-            next
-              case False
-              with predfss u have "u \<in> explored e \<union> \<S> e (hd (stack e))"
-                by (auto simp: pre_dfss_def)
-              then show ?thesis
-              proof
-                assume "u \<in> explored e"
-                with postdfsw show ?thesis
-                  by (auto simp: post_dfs_def sub_env_def)
-              next
-                assume u: "u \<in> \<S> e (hd (stack e))"
-                from predfss have "stack e \<noteq> []"
-                  by (simp add: pre_dfss_def)
-                with u have "u \<in> \<Union> {\<S> e n | n . n \<in> set (stack e)}"
-                  by force
-                moreover
-                from postdfsw have "sub_env e e'"
-                  by (simp add: post_dfs_def)
-                ultimately obtain n where
-                  n: "n \<in> set (stack e')" "u \<in> \<S> e' n"
-                  using u unfolding sub_env_def by blast
-                have "n = hd (stack e')"
-                proof (rule ccontr)
-                  assume "n \<noteq> hd (stack e')"
-                  with postdfsw n \<open>stack e' \<noteq> []\<close> 
-                  have "\<S> e' n = \<S> e n"
-                    unfolding post_dfs_def by (metis hd_Cons_tl set_ConsD)
-                  moreover
-                  from n \<open>n \<noteq> hd (stack e')\<close> \<open>stack e' \<noteq> []\<close>
-                       \<open>\<exists>ns. stack e = ns @ (stack e')\<close>
-                  have "n \<in> set (tl (stack e))"
-                    by (metis Un_iff append_Nil hd_Cons_tl set_ConsD set_append tl_append2)
-                  ultimately show "False"
-                    using u n \<open>stack e \<noteq> []\<close> predfss
-                    unfolding pre_dfss_def wf_env_def
-                    by (metis (no_types, opaque_lifting) Diff_cancel Diff_triv distinct.simps(2) empty_iff list.exhaust_sel list.set_sel(1) list.set_sel(2))
-                qed
-                with n show ?thesis by simp
-              qed
-            qed
-          }
+          from wf' wvs have "\<forall>v. vsuccs e'' v \<subseteq> successors v"
+            by (auto simp: wf_env_def e''_def)
+          moreover 
+          from wf' True have "\<forall>v. vsuccs e'' v \<subseteq> visited e''"
+            by (auto simp: wf_env_def e''_def e')
+          moreover
+          from wf' \<open>v \<in> visited e\<close>
+          have "\<forall>v. v \<notin> visited e'' \<longrightarrow> vsuccs e'' v = {}"
+            by (auto simp: wf_env_def e''_def e')
+          moreover
+          from wf' wvs
+          have "\<forall>v. v \<in> explored e'' \<longrightarrow> vsuccs e'' v = successors v"
+            by (auto simp: wf_env_def e''_def)
+          moreover
+          have "\<forall>x y. x \<preceq> y in stack e'' \<and> x \<noteq> y \<longrightarrow>
+                   (\<forall>u \<in> \<S> e'' x. \<not> reachable_avoiding u y (unvisited e'' x))"
+          proof (clarify)
+            fix x y u
+            assume "x \<preceq> y in stack e''" "x \<noteq> y" 
+                   "u \<in> \<S> e'' x"
+                   "reachable_avoiding u y (unvisited e'' x)"
+            show "False"
+              sorry
+          qed
+          ultimately show ?thesis
+            unfolding wf_env_def by blast
+        qed
+        with True predfss
+        have "pre_dfss v e''"
+          by (auto simp: pre_dfss_def e''_def e')
+        with prepostdfss vs_case have post'': "post_dfss v e'' (dfss v e'')"
+          by (auto simp: w_def e'_def e''_def)
 
-          moreover have "v \<in> \<S> e' (hd (stack e'))"
+        moreover
+        from post''
+        have "\<forall>u \<in> visited e - {v}. vsuccs (dfss v e'') u = vsuccs e u"
+          by (auto simp: post_dfss_def e' e''_def)
+
+        moreover
+        have "sub_env e e''"
+          by (auto simp: sub_env_def e' e''_def)
+        with post'' have "sub_env e (dfss v e'')"
+          by (auto simp: post_dfss_def elim: sub_env_trans)
+
+        moreover
+        from e' have "stack e'' = stack e" "\<S> e'' = \<S> e"
+          by (auto simp add: e''_def)
+
+        ultimately show ?thesis
+          by (auto simp: dfss post_dfss_def)
+      next
+        case notexplored: False
+        then show ?thesis
+        proof (cases "w \<notin> visited e")
+          case True
+          hence "e' = dfs w e" using e'_def notexplored
+            by auto
+          with True notexplored pre_dfss_pre_dfs predfss prepostdfs vs_case w_def
+          have postdfsw: "post_dfs w e e'"
+            by (metis DiffD1 some_in_eq)
+
+          from postdfsw have "w \<in> visited e'"
+            unfolding post_dfs_def wf_env_def by blast
+          from predfss postdfsw have "stack e' \<noteq> []"
+            by (auto simp: pre_dfss_def post_dfs_def)
+          have "v \<in> \<S> e' (hd (stack e'))"
           proof (cases "stack e' = stack e")
             case True
-            then show ?thesis
-              by (metis post_dfs_def postdfsw pre_dfss_def predfss sub_env_def subset_iff)
+            with predfss postdfsw show ?thesis
+              unfolding pre_dfss_def post_dfs_def sub_env_def
+              by (metis subsetD)
           next
             case False
             with postdfsw have se': "w \<in> \<S> e' (hd (stack e'))" "\<forall>n \<in> set (tl (stack e')). \<S> e' n = \<S> e n"
@@ -1466,7 +1307,8 @@ next
               by (auto simp: pre_dfss_def)
             with postdfsw obtain n where
               n: "n \<in> set (stack e')" "v \<in> \<S> e' n"
-              unfolding post_dfs_def sub_env_def by blast
+              unfolding post_dfs_def sub_env_def
+              by (smt (verit, ccfv_threshold) Union_iff mem_Collect_eq subsetD)
             show ?thesis
             proof (cases "n = hd (stack e')")
               case True
@@ -1489,301 +1331,562 @@ next
             qed
           qed
 
-          moreover
-          {
-            fix n u
-            assume asm: "hd (stack e') = v"
-                        "n \<in> set (tl (stack e'))" "u \<in> \<S> e' (hd (stack e')) - {v}"
-                        "reachable_avoiding u n (\<S> e' (hd (stack e')))"
-            from postdfsw obtain ns where "stack e = ns @ (stack e')"
-              unfolding post_dfs_def by blast
-            with \<open>stack e' \<noteq> []\<close> \<open>hd (stack e') = v\<close> predfss
-            have "hd (stack e) = v"
-              unfolding pre_dfss_def wf_env_def
-              by (smt (z3) Un_iff disjoint_iff list.set_sel(1) set_append)
-            with \<open>stack e = ns @ (stack e')\<close> \<open>hd (stack e') = v\<close> \<open>stack e' \<noteq> []\<close> predfss
-            have "stack e' = stack e" 
-              unfolding pre_dfss_def wf_env_def
-              by (metis self_append_conv2 suffix_same_head)
-            have "False"
-            proof (cases "u \<in> \<S> e (hd (stack e'))")
-              case True
-              from \<open>reachable_avoiding u n (\<S> e' (hd (stack e')))\<close> postdfsw
-              have "reachable_avoiding u n (\<S> e (hd (stack e')))"
-                unfolding post_dfs_def sub_env_def using ra_mono by auto
-              with asm predfss \<open>stack e' = stack e\<close> True show ?thesis
-                unfolding pre_dfss_def by auto
-            next
-              case False
-              with asm predfss postdfsw \<open>stack e' = stack e\<close> show ?thesis
-                by (auto simp: pre_dfss_def post_dfs_def)
-            qed
-          }
-
-          ultimately show ?thesis
-            unfolding pre_dfss_def by blast
-        qed
-
-        moreover have "post_dfss v (vs - {w}) e' (dfss v (vs - {w}) e')"
-          using True \<open>e' = dfs w e\<close> calculation notexplored prepostdfss vs_case w_def by auto
-
-        moreover have almost:"post_dfss v (vs - {w}) e' (dfss v vs e)"
-          using calculation(2) calculation(4) by simp
-
-        with postdfsw have "\<forall> w \<in> vs. \<forall> x. reachable w x \<longrightarrow> x \<in> visited (dfss v vs e)"
-          by (auto simp: post_dfss_def post_dfs_def sub_env_def)
-
-        moreover have "sub_env e (dfss v vs e)"
-        proof -
-          have "sub_env e e'"
-            using post_dfs_def postdfsw by blast
-          moreover have "sub_env e' (dfss v vs e)"
-            using almost post_dfss_def by blast
-          ultimately show ?thesis
-            by (meson order_trans sub_env_def)
-        qed
-  
-        moreover have "\<exists> ns. stack e = ns @ (stack (dfss v vs e))"
-        proof -
-          have "\<exists> ns. stack e = ns @ (stack e')"
-            using post_dfs_def postdfsw by blast
-          moreover have "\<exists> ns. stack e' = ns @ (stack (dfss v vs e))"
-            using almost post_dfss_def by blast
-          ultimately show ?thesis
-            by fastforce
-        qed
-
-        moreover
-        {
-          fix n
-          assume n: "n \<in> set (tl (stack (dfss v vs e)))"
-          with almost have "\<S> (dfss v vs e) n = \<S> e' n"
-            by (auto simp: post_dfss_def)
-          moreover
-          from almost n have "stack e' \<noteq> [] \<and> n \<in> set (tl (stack e'))"
-            unfolding post_dfss_def
-            by (metis Nil_is_append_conv Un_iff list.set_sel(2) self_append_conv2 set_append tl_append2)
-          with postdfsw have "\<S> e' n = \<S> e n"
-            unfolding post_dfs_def
-            by (metis list.set_sel(2))
-          ultimately have "\<S> (dfss v vs e) n = \<S> e n"
-            by simp
-        }
-
-        ultimately show ?thesis
-          by (simp add: post_dfss_def)
-      next
-        case False
-        hence "e' = unite v w e" using notexplored
-          using e'_def by simp
-        from False have "w \<in> visited e"
-          by simp
-        from predfss have "wf_env e"
-          by (simp add: pre_dfss_def)
-
-        define pfx where "pfx = takeWhile (\<lambda>x. w \<notin> \<S> e x) (stack e)"
-        define sfx where "sfx = dropWhile (\<lambda>x. w \<notin> \<S> e x) (stack e)"
-        define cc where "cc = \<Union> {\<S> e x |x. x \<in> set pfx \<union> {hd sfx}}"
-
-        have "stack e = pfx @ sfx"
-            by (simp add: pfx_def sfx_def)
-
-        have tl_sfx_not_in_cc:"\<forall> x \<in> set (tl sfx). x \<notin> cc"
-        proof (clarify)
-          fix x
-          assume asm:"x \<in> set (tl sfx)" "x \<in> cc"
-          from asm(2) obtain n where n_def:"n \<in> set pfx \<union> {hd sfx}" "x \<in> \<S> e n" using cc_def
-            by blast
-          have "n \<in> set (stack e)" using \<open>stack e = pfx @ sfx\<close> asm(1)
-            by (metis Un_iff empty_set equals0D hd_in_set insertE list.sel(2) n_def(1) set_append)
-          moreover have "x \<in> set (stack e)" using asm(1)
-            by (metis list.sel(2) list.set_sel(2) set_dropWhileD sfx_def)
-          moreover have "x \<noteq> n"
-            by (smt (verit, best) IntI Un_iff \<open>stack e = pfx @ sfx\<close> asm(1) distinct.simps(2) distinct_append empty_iff empty_set list.exhaust_sel list.sel(2) list.set_sel(2) n_def(1) pre_dfss_def predfss singletonD wf_env_def)
-          moreover have "\<S> e x \<inter> \<S> e n \<noteq> {}"
-            by (smt (verit, best) equals0D inf_idem n_def(2) pre_dfss_def predfss wf_env_def)
-          ultimately show False using predfss
-            by (simp add: pre_dfss_def wf_env_def)
-        qed
-
-        obtain ww where ww_def: "ww \<in> set (stack e) \<and> w \<in> \<S> e ww" 
-          using notexplored \<open>w \<in> visited e\<close> predfss unfolding pre_dfss_def wf_env_def
-          by (smt (verit, ccfv_threshold) DiffI UnionE mem_Collect_eq)
-        hence "ww \<in> set sfx"
-          by (metis Un_iff set_append set_takeWhileD sfx_def takeWhile_dropWhile_id)
-        hence "sfx \<noteq> []"
-          by auto
-        have "ww = hd sfx"
-        proof (rule ccontr)
-          assume "ww \<noteq> hd sfx"
-          from \<open>ww \<in> set sfx\<close> have "w \<in> \<S> e (hd sfx)"
-            unfolding sfx_def by (metis empty_iff empty_set hd_dropWhile)
-          with ww_def \<open>wf_env e\<close> \<open>sfx \<noteq> []\<close> \<open>stack e = pfx @ sfx\<close> \<open>ww \<noteq> hd sfx\<close> 
-          show "False"
-            unfolding wf_env_def
-            by (metis (no_types, lifting) Diff_cancel Diff_triv Un_iff insert_Diff insert_not_empty list.set_sel(1) set_append)
-        qed
-        with ww_def have "w \<in> \<S> e (hd sfx)"
-          by simp
-
-        have cc_scc: "is_subscc cc"
-        proof (clarsimp simp: is_subscc_def)
-          fix x y
-          assume "x \<in> cc" "y \<in> cc"
-          then obtain nx ny where
-            nx: "nx \<in> set pfx \<union> {hd sfx}" "x \<in> \<S> e nx" and
-            ny: "ny \<in> set pfx \<union> {hd sfx}" "y \<in> \<S> e ny"
-            by (auto simp: cc_def)
-          with \<open>wf_env e\<close>
-          have "reachable x nx" "reachable ny y"
-            by (auto simp: wf_env_def is_subscc_def)
-          from wvs predfss have "reachable v w"
-            by (auto simp: pre_dfss_def)
-          from predfss 
-          have "reachable (hd (stack e)) v"
-            by (auto simp: pre_dfss_def wf_env_def is_subscc_def)
-          from predfss have "stack e = hd (stack e) # tl (stack e)"
-            by (auto simp: pre_dfss_def)
-          with nx \<open>stack e = pfx @ sfx\<close> \<open>sfx \<noteq> []\<close>
-          have "hd (stack e) \<preceq> nx in stack e"
-            by (metis Un_iff Un_insert_right head_precedes list.exhaust_sel list.simps(15) set_append sup_bot.right_neutral)
-          with \<open>wf_env e\<close> have "reachable nx (hd (stack e))"
-            by (auto simp: wf_env_def)
-          from \<open>stack e = pfx @ sfx\<close> \<open>sfx \<noteq> []\<close> \<open>ww = hd sfx\<close> ny
-          have "ny \<preceq> ww in stack e" 
-            by (metis List.set_insert empty_set insert_Nil list.exhaust_sel set_append split_list_precedes)
-          with \<open>wf_env e\<close> have "reachable ww ny"
-            by (auto simp: wf_env_def is_subscc_def)
-          from ww_def \<open>wf_env e\<close> have "reachable w ww"
-            by (auto simp: wf_env_def is_subscc_def)
-
-          from \<open>reachable x nx\<close> \<open>reachable nx (hd (stack e))\<close>
-               \<open>reachable (hd (stack e)) v\<close> \<open>reachable v w\<close>
-               \<open>reachable w ww\<close> \<open>reachable ww ny\<close> \<open>reachable ny y\<close>
-          show "reachable x y"
-            using reachable_trans by meson
-        qed
-
-        have e'_def: "e' = e\<lparr>\<S> := \<lambda>x. if x \<in> cc then cc else \<S> e x, stack := sfx\<rparr>" using unite_def
-          using \<open>e' = unite v w e\<close> cc_def pfx_def sfx_def by auto
-
-        from \<open>sfx \<noteq> []\<close> have "stack e' = (hd sfx) # tl sfx"
-          by (auto simp: e'_def)
-        moreover
-        from \<open>wf_env e\<close> \<open>sfx \<noteq> []\<close> have "\<S> e' (hd sfx) = cc"
-          by (auto simp: wf_env_def cc_def e'_def)
-        moreover
-        from tl_sfx_not_in_cc have "\<forall>v \<in> set (tl sfx). \<S> e' v = \<S> e v"
-          by (simp add: e'_def)
-        ultimately
-        have "(\<Union> {\<S> e' v | v. v \<in> set (stack e')}) 
-              = cc \<union> (\<Union> {\<S> e v | v. v \<in> set (tl sfx)})"
-          by auto
-        moreover
-        from \<open>stack e = pfx @ sfx\<close> \<open>sfx \<noteq> []\<close>
-        have "stack e = pfx @ (hd sfx # tl sfx)"
-          by auto
-        ultimately
-        have s_equal: "(\<Union> {\<S> e' v | v. v \<in> set (stack e')}) 
-                       = (\<Union> {\<S> e v | v. v \<in> set (stack e)})"
-          by (auto simp: cc_def)
-
-        have "\<exists>ns. stack e = ns @ (stack e')" 
-          using \<open>stack e = pfx @ sfx\<close> by (simp add: e'_def)
-
-        moreover have "sub_env e e'"
-        proof -
-          have "\<forall> x. \<S> e x \<subseteq> \<S> e' x"
+          have "wf_env e''"
           proof -
+            from postdfsw have wf': "wf_env e'"
+              by (simp add: post_dfs_def)
+            hence "distinct (stack e'')"
+                  "set (stack e'') \<subseteq> visited e''"
+                  "explored e'' \<subseteq> visited e''"
+                  "explored e'' \<inter> set (stack e'') = {}"
+                  "\<forall>v w. w \<in> \<S> e'' v \<longleftrightarrow> (\<S> e'' v = \<S> e'' w)"
+                  "\<forall>v \<in> set (stack e''). \<forall> w \<in> set (stack e''). 
+                      v \<noteq> w \<longrightarrow> \<S> e'' v \<inter> \<S> e'' w = {}"
+                  "\<forall> v. v \<notin> visited e'' \<longrightarrow> \<S> e'' v = {v}"
+                  "\<Union> {\<S> e'' v | v. v \<in> set (stack e'')} = visited e'' - explored e''"
+                  "\<forall>x y. x \<preceq> y in stack e'' \<longrightarrow> reachable y x"
+                  "\<forall>x. is_subscc (\<S> e'' x)"
+                  "\<forall> x \<in> explored e''. \<forall> y. reachable x y \<longrightarrow> y \<in> explored e''"
+                  "\<forall> S \<in> sccs e''. is_scc S"
+              by (auto simp: wf_env_def e''_def)
+            moreover
+            from wf' wvs have "\<forall>v. vsuccs e'' v \<subseteq> successors v"
+              by (auto simp: wf_env_def e''_def)
+            moreover 
+            from wf' \<open>w \<in> visited e'\<close> have "\<forall>v. vsuccs e'' v \<subseteq> visited e''"
+              by (auto simp: wf_env_def e''_def)
+            moreover
+            have "\<forall>u. u \<notin> visited e'' \<longrightarrow> vsuccs e'' u = {}"
+            proof (clarify)
+              fix u
+              assume u: "u \<notin> visited e''"
+              with \<open>v \<in> visited e\<close> postdfsw have "u \<noteq> v"
+                by (auto simp: post_dfs_def sub_env_def e''_def)
+              moreover
+              from u wf' have "vsuccs e' u = {}"
+                by (auto simp: wf_env_def e''_def)
+              ultimately show "vsuccs e'' u = {}"
+                by (simp add: e''_def)
+            qed
+            moreover
+            from wf' wvs
+            have "\<forall>v. v \<in> explored e'' \<longrightarrow> vsuccs e'' v = successors v"
+              by (auto simp: wf_env_def e''_def)
+            moreover
+            have "\<forall>x y. x \<preceq> y in stack e'' \<and> x \<noteq> y \<longrightarrow>
+                     (\<forall>u \<in> \<S> e'' x. \<not> reachable_avoiding u y (unvisited e'' x))"
+            proof (clarify)
+              fix x y u
+              assume "x \<preceq> y in stack e''" "x \<noteq> y"
+                     "u \<in> \<S> e'' x"
+                     "reachable_avoiding u y (unvisited e'' x)"
+              show "False"
+                sorry
+            qed
+            ultimately show ?thesis
+              unfolding wf_env_def by blast
+          qed
+
+          have "pre_dfss v e''"
+          proof -
+            from predfss postdfsw
+            have "v \<in> visited e''"
+              by (auto simp: pre_dfss_def post_dfs_def sub_env_def e''_def)
+            moreover
             {
-              fix x
-              have "\<S> e x \<subseteq> \<S> e' x"
-              proof (cases "x \<in> (set pfx) \<union> {hd sfx}")
+              fix u
+              assume u: "u \<in> vsuccs e'' v"
+              have "u \<in> explored e'' \<union> \<S> e'' (hd (stack e''))"
+              proof (cases "u = w")
                 case True
-                hence "\<S> e x \<subseteq> cc"
-                  using cc_def by auto
-                then show ?thesis using e'_def
-                  by simp
+                with postdfsw show ?thesis
+                  by (auto simp: post_dfs_def e''_def)
               next
-                case xFalse:False
+                case False
+                with u predfss postdfsw
+                have "u \<in> explored e \<union> \<S> e (hd (stack e))"
+                  by (auto simp: pre_dfss_def post_dfs_def e''_def)
                 then show ?thesis
-                proof (cases "x \<in> set (tl sfx)")
-                  case True
-                  hence "x \<notin> cc"
-                  proof -
-                    have "x \<in> set (stack e)" using True
-                      by (metis \<open>ww \<in> set sfx\<close> empty_iff list.set_sel(2) set_dropWhileD set_empty2 sfx_def)
-                    {
-                      fix y
-                      assume asm:"y \<in> set (pfx) \<or> y = hd sfx"
-                      hence "x \<notin> \<S> e y"
-                      proof (cases "y = hd sfx")
-                        case True
-                        hence "x \<noteq> y"
-                          using xFalse by auto
-                        then show ?thesis using predfss pre_dfss_def wf_env_def
-                          by (smt (verit, ccfv_threshold) True \<open>ww \<in> set sfx\<close> \<open>x \<in> set (stack e)\<close> empty_iff empty_set inf.idem list.set_sel(1) set_dropWhileD sfx_def)
-                      next  
-                        case False
-                        hence "y \<in> set pfx"
-                          using asm by blast
-                        then show ?thesis using True \<open>stack e = pfx @ sfx\<close> using \<open>x \<in> set (stack e)\<close> predfss unfolding pre_dfss_def wf_env_def
-                        by (metis (mono_tags, lifting) xFalse UnI1 equals0D inf.idem pfx_def set_takeWhileD)
-                      qed
-                    }
-                    then show ?thesis
-                      using cc_def by blast
-                  qed
-                  then show ?thesis
-                    by (simp add: e'_def)
+                proof
+                  assume "u \<in> explored e"
+                  with postdfsw show ?thesis
+                    by (auto simp: post_dfs_def sub_env_def e''_def)
                 next
-                  case False
-                  hence "x \<notin> set (stack e)" using xFalse \<open>stack e = pfx @ sfx\<close>
-                    by (metis Un_iff empty_set insert_iff list.exhaust_sel list.simps(15) set_append)
-                  moreover have "stack e' = sfx" using e'_def
-                    by simp
-                  hence "x \<notin> set (stack e')"
-                    using calculation set_dropWhileD sfx_def by fastforce
-                  have "\<S> e' x = cc \<or> \<S> e x = \<S> e' x" using e'_def
-                    by simp
-                  then show ?thesis
-                  proof (cases "\<S> e' x = cc")
-                    case True
-                    then show ?thesis
-                    proof (cases "x \<in> visited e")
-                      case True
-                      then show ?thesis
-                        by (smt (verit, ccfv_threshold) cc_def e'_def ext_inject mem_Collect_eq mem_simps(9) pre_dfss_def predfss subsetI surjective update_convs(1) update_convs(5) wf_env_def)
-                    next
-                      case False
-                      then show ?thesis
-                        using e'_def pre_dfss_def predfss wf_env_def by fastforce
-                    qed
-                  next
-                    case False
-                    then show ?thesis
-                      using \<open>\<S> e' x = cc \<or> \<S> e x = \<S> e' x\<close> by force
+                  assume "u \<in> \<S> e (hd (stack e))"
+                  from predfss have "hd (stack e) \<in> set (stack e)"
+                    by (auto simp: pre_dfss_def)
+                  with \<open>u \<in> \<S> e (hd (stack e))\<close>
+                  have "u \<in> \<Union> {\<S> e v | v . v \<in> set (stack e)}"
+                    by auto
+                  with postdfsw obtain n where
+                    n: "n \<in> set (stack e')" "u \<in> \<S> e' n"
+                    unfolding post_dfs_def sub_env_def
+                    by (smt (verit, ccfv_threshold) Union_iff mem_Collect_eq subsetD)
+                  have "n = hd (stack e')"
+                  proof (rule ccontr)
+                    assume "n \<noteq> hd (stack e')"
+                    with n \<open>stack e' \<noteq> []\<close> postdfsw
+                    have "n \<in> set (tl (stack e)) \<and> \<S> e' n = \<S> e n"
+                      unfolding post_dfs_def
+                      by (metis Un_iff list.exhaust_sel self_append_conv2 set_ConsD set_append tl_append2)
+                    with predfss \<open>u \<in> \<S> e (hd (stack e))\<close> \<open>u \<in> \<S> e' n\<close>
+                    show "False"
+                      unfolding pre_dfss_def wf_env_def
+                      by (metis (no_types, lifting) distinct.simps(2) insert_Diff insert_disjoint(2) list.exhaust_sel list.set_sel(1) list.set_sel(2))
                   qed
+                  with n show ?thesis
+                    by (simp add: e''_def)
                 qed
               qed
             }
-            then show ?thesis
-              by fastforce
+            moreover
+            from predfss postdfsw 
+            have "\<forall>n \<in> set (stack e''). reachable n v"
+              unfolding pre_dfss_def post_dfs_def
+              using e''_def by force
+            moreover
+            from \<open>stack e' \<noteq> []\<close> have "stack e'' \<noteq> []"
+              by (simp add: e''_def)
+            moreover
+            from \<open>v \<in> \<S> e' (hd (stack e'))\<close> have "v \<in> \<S> e'' (hd (stack e''))"
+              by (simp add: e''_def)
+            ultimately show ?thesis
+              using \<open>wf_env e''\<close>
+              unfolding pre_dfss_def by blast
           qed
-          with s_equal show ?thesis
-            by (simp add: sub_env_def e'_def)
-        qed
 
-      moreover have "pre_dfss v (vs - {w}) e'"
+          with prepostdfss vs_case 
+          have post'': "post_dfss v e'' (dfss v e'')"
+            by (auto simp: w_def e'_def e''_def)
+
+          moreover
+          have "\<forall>u \<in> visited e - {v}. vsuccs (dfss v e'') u = vsuccs e u"
+          proof
+            fix u
+            assume "u \<in> visited e - {v}"
+            with postdfsw 
+            have u: "vsuccs e' u = vsuccs e u" "u \<in> visited e'' - {v}"
+              by (auto simp: post_dfs_def sub_env_def e''_def)
+            with post'' have "vsuccs (dfss v e'') u = vsuccs e'' u"
+              by (auto simp: post_dfss_def)
+            with u show "vsuccs (dfss v e'') u = vsuccs e u"
+              by (simp add: e''_def)
+          qed
+
+          moreover
+          have "sub_env e (dfss v e'')"
+          proof -
+            from postdfsw have "sub_env e e'"
+              by (simp add: post_dfs_def)
+            moreover
+            have "sub_env e' e''"
+              by (auto simp: sub_env_def e''_def)
+            moreover
+            from post'' have "sub_env e'' (dfss v e'')"
+              by (simp add: post_dfss_def)
+            ultimately show ?thesis
+              using sub_env_trans by metis
+          qed
+
+          moreover
+          have "\<exists>ns. stack e = ns @ (stack (dfss v e''))"
+          proof -
+            from postdfsw obtain xs where "stack e = xs @ stack e''"
+              by (auto simp: post_dfs_def e''_def)
+            moreover
+            from post'' obtain ys where "stack e'' = ys @ stack (dfss v e'')"
+              by (auto simp: post_dfss_def)
+            ultimately show ?thesis
+              by auto
+          qed
+
+          moreover
+          {
+            fix n
+            assume n: "n \<in> set (tl (stack (dfss v e'')))"
+            with post'' have "\<S> (dfss v e'') n = \<S> e' n"
+              by (simp add: post_dfss_def e''_def)
+            moreover
+            from n post'' have "n \<in> set (tl (stack e''))"
+              unfolding post_dfss_def
+              by (metis Un_iff list.set_sel(2) self_append_conv2 set_append tl_append2)
+            with postdfsw e''_def have "\<S> e' n = \<S> e n"
+              unfolding post_dfs_def
+              by (metis (no_types, lifting) list.sel(2) list.set_sel(2) select_convs(6) simps(11) surjective)
+            ultimately have "\<S> (dfss v e'') n = \<S> e n"
+              by simp
+          }
+
+          ultimately show ?thesis
+            by (auto simp: dfss post_dfss_def)
+
+        next
+          case False
+          hence "e' = unite v w e" using notexplored
+            using e'_def by simp
+          from False have "w \<in> visited e"
+            by simp
+          from predfss have "wf_env e"
+            by (simp add: pre_dfss_def)
+
+          define pfx where "pfx = takeWhile (\<lambda>x. w \<notin> \<S> e x) (stack e)"
+          define sfx where "sfx = dropWhile (\<lambda>x. w \<notin> \<S> e x) (stack e)"
+          define cc where "cc = \<Union> {\<S> e x |x. x \<in> set pfx \<union> {hd sfx}}"
+
+          have "stack e = pfx @ sfx"
+            by (simp add: pfx_def sfx_def)
+
+          have cc_Un: "cc = \<Union> {\<S> e x | x. x \<in> cc}"
+            sorry
+
+          from \<open>wf_env e\<close> \<open>w \<in> visited e\<close> \<open>w \<notin> explored e\<close>
+          obtain n where "n \<in> set (stack e) \<and> w \<in> \<S> e n"
+            unfolding wf_env_def
+            by (smt (verit, del_insts) Diff_iff Union_iff mem_Collect_eq)
+          hence sfx: "sfx \<noteq> [] \<and> w \<in> \<S> e (hd sfx)"
+            unfolding sfx_def
+            by (metis dropWhile_eq_Nil_conv hd_dropWhile)
+          with \<open>wf_env e\<close> \<open>stack e = pfx @ sfx\<close> 
+          have pfx: "set pfx \<union> {hd sfx} \<subseteq> cc"
+            unfolding wf_env_def cc_def 
+            by (smt (verit) Union_iff mem_Collect_eq subset_eq)
+          have tl_int_cc: "\<forall>n \<in> set (tl sfx). \<S> e n \<inter> cc = {}"
+          proof -
+            {
+              fix n u
+              assume "n \<in> set (tl sfx)" "u \<in> \<S> e n" "u \<in> cc"
+              from sfx \<open>n \<in> set (tl sfx)\<close> \<open>stack e = pfx @ sfx\<close> \<open>wf_env e\<close>
+              have n: "n \<in> set (stack e) - (set pfx \<union> {hd sfx})"
+                unfolding wf_env_def
+                by (metis Diff_iff Int_iff Un_iff distinct.simps(2) distinct_append empty_iff list.exhaust_sel list.set_sel(2) set_append singletonD)
+              from \<open>u \<in> cc\<close> obtain n' where
+                n': "n' \<in> set pfx \<union> {hd sfx}" "u \<in> \<S> e n'"
+                by (auto simp: cc_def)
+              with n \<open>stack e = pfx @ sfx\<close> sfx \<open>wf_env e\<close>
+              have "\<S> e n \<inter> \<S> e n' = {}"
+                unfolding wf_env_def
+                by (metis (no_types, lifting) DiffE UnCI UnE list.set_sel(1) set_append singleton_iff)
+              with \<open>u \<in> \<S> e n\<close> \<open>u \<in> \<S> e n'\<close> have "False"
+                by auto
+            }
+            thus ?thesis by auto
+          qed
+
+          with \<open>wf_env e\<close> sfx \<open>stack e = pfx @ sfx\<close>
+          have tl_sfx_not_in_cc: "\<forall> x \<in> set (tl sfx). x \<notin> cc"
+            unfolding wf_env_def cc_def
+            by (metis (no_types, lifting) disjoint_insert(1) insert_Diff)
+
+          have cc_scc: "is_subscc cc"
+          proof (clarsimp simp: is_subscc_def)
+            fix x y
+            assume "x \<in> cc" "y \<in> cc"
+            then obtain nx ny where
+              nx: "nx \<in> set pfx \<union> {hd sfx}" "x \<in> \<S> e nx" and
+              ny: "ny \<in> set pfx \<union> {hd sfx}" "y \<in> \<S> e ny"
+              by (auto simp: cc_def)
+            with \<open>wf_env e\<close>
+            have "reachable x nx" "reachable ny y"
+              by (auto simp: wf_env_def is_subscc_def)
+            from wvs predfss have "reachable v w"
+              by (auto simp: pre_dfss_def)
+            from predfss 
+            have "reachable (hd (stack e)) v"
+              by (auto simp: pre_dfss_def wf_env_def is_subscc_def)
+            from predfss have "stack e = hd (stack e) # tl (stack e)"
+              by (auto simp: pre_dfss_def)
+            with nx \<open>stack e = pfx @ sfx\<close> sfx
+            have "hd (stack e) \<preceq> nx in stack e"
+              by (metis Un_iff Un_insert_right head_precedes list.exhaust_sel list.simps(15) set_append sup_bot.right_neutral)
+            with \<open>wf_env e\<close> have "reachable nx (hd (stack e))"
+              by (auto simp: wf_env_def)
+            from \<open>stack e = pfx @ sfx\<close> sfx ny
+            have "ny \<preceq> hd sfx in stack e" 
+              by (metis List.set_insert empty_set insert_Nil list.exhaust_sel set_append split_list_precedes)
+            with \<open>wf_env e\<close> have "reachable (hd sfx) ny"
+              by (auto simp: wf_env_def is_subscc_def)
+            from sfx \<open>wf_env e\<close> have "reachable w (hd sfx)"
+              by (auto simp: wf_env_def is_subscc_def)
+
+            from \<open>reachable x nx\<close> \<open>reachable nx (hd (stack e))\<close>
+                 \<open>reachable (hd (stack e)) v\<close> \<open>reachable v w\<close>
+                 \<open>reachable w (hd sfx)\<close> \<open>reachable (hd sfx) ny\<close> \<open>reachable ny y\<close>
+            show "reachable x y"
+              using reachable_trans by meson
+          qed
+
+          have e'_def: "e' = e\<lparr>\<S> := \<lambda>x. if x \<in> cc then cc else \<S> e x, stack := sfx\<rparr>" using unite_def
+            using \<open>e' = unite v w e\<close> cc_def pfx_def sfx_def by auto
+
+          from pfx have hd_sfx: "\<S> e' (hd sfx) = cc"
+            by (simp add: e'_def)
+
+          from tl_sfx_not_in_cc tl_int_cc
+          have tl_sfx: "\<forall>x \<in> set (tl sfx). \<S> e' x = \<S> e x \<and> \<S> e' x \<inter> cc = {}"
+            by (simp add: e'_def)
+
+          from sfx have "stack e' = (hd sfx) # tl sfx"
+            by (auto simp: e'_def)
+          moreover
+          from tl_sfx_not_in_cc have "\<forall>v \<in> set (tl sfx). \<S> e' v = \<S> e v"
+            by (simp add: e'_def)
+          ultimately
+          have "(\<Union> {\<S> e' v | v. v \<in> set (stack e')}) 
+                = cc \<union> (\<Union> {\<S> e v | v. v \<in> set (tl sfx)})"
+            using hd_sfx by auto
+          moreover
+          from \<open>stack e = pfx @ sfx\<close> sfx
+          have "stack e = pfx @ (hd sfx # tl sfx)"
+            by auto
+          ultimately
+          have s_equal: "(\<Union> {\<S> e' v | v. v \<in> set (stack e')}) 
+                         = (\<Union> {\<S> e v | v. v \<in> set (stack e)})"
+            by (auto simp: cc_def)
+
+          have "\<exists>ns. stack e = ns @ (stack e')" 
+            using \<open>stack e = pfx @ sfx\<close> by (simp add: e'_def)
+
+          moreover have "sub_env e e'"
+          proof -
+            have "\<forall> x. \<S> e x \<subseteq> \<S> e' x"
+            proof
+              fix x
+              show "\<S> e x \<subseteq> \<S> e' x"
+              proof (cases "x \<in> cc")
+                case True
+                then obtain n where
+                  n: "n \<in> set pfx \<union> {hd sfx}" "x \<in> \<S> e n"
+                  by (auto simp: cc_def)
+                with \<open>wf_env e\<close> have "\<S> e x = \<S> e n"
+                  by (auto simp: wf_env_def)
+                with \<open>n \<in> set pfx \<union> {hd sfx}\<close> have "\<S> e x \<subseteq> cc"
+                  by (auto simp: cc_def)
+                moreover
+                from n have "x \<in> cc"
+                  by (auto simp: cc_def)
+                ultimately show ?thesis
+                  by (simp add: e'_def)
+              next
+                case False
+                then show ?thesis
+                  by (simp add: e'_def)
+              qed
+            qed
+            with s_equal show ?thesis
+              by (simp add: sub_env_def e'_def)
+          qed
+
+          have "wf_env e''"
+          proof -
+            from \<open>wf_env e\<close> \<open>stack e = pfx @ sfx\<close>
+            have "distinct (stack e'')" 
+                 "set (stack e'') \<subseteq> visited e''" 
+                 "explored e'' \<subseteq> visited e''"
+                 "explored e'' \<inter> set (stack e'') = {}"
+              by (auto simp: wf_env_def e'_def e''_def)
+
+            moreover
+            from \<open>wf_env e\<close> wvs
+            have "\<forall>x. vsuccs e'' x \<subseteq> successors x"
+              by (simp add: wf_env_def e'_def e''_def)
+
+            moreover
+            from \<open>wf_env e\<close> \<open>w \<in> visited e\<close>
+            have "\<forall>x. vsuccs e'' x \<subseteq> visited e''"
+              by (simp add: wf_env_def e'_def e''_def)
+
+            moreover
+            from \<open>wf_env e\<close> \<open>w \<in> visited e\<close> \<open>v \<in> visited e\<close>
+            have "\<forall>x. x \<notin> visited e'' \<longrightarrow> vsuccs e'' x = {}"
+              by (simp add: wf_env_def e'_def e''_def)
+
+            moreover
+            from \<open>wf_env e\<close> \<open>v \<notin> explored e\<close>
+            have "\<forall>x. x \<in> explored e'' \<longrightarrow> vsuccs e'' x = successors x"
+              by (simp add: wf_env_def e'_def e''_def)
+
+            moreover
+            {
+              fix x y
+              have "y \<in> \<S> e' x \<longleftrightarrow> (\<S> e' x = \<S> e' y)"
+              proof
+                assume y: "y \<in> \<S> e' x"
+                show "\<S> e' x = \<S> e' y"
+                proof (cases "x \<in> cc")
+                  case True
+                  with y show ?thesis
+                    by (simp add: e'_def)
+                next
+                  case False
+                  with y \<open>wf_env e\<close> have "\<S> e x = \<S> e y"
+                    by (simp add: wf_env_def e'_def)
+                  with False cc_Un \<open>wf_env e\<close> have "y \<notin> cc"
+                    unfolding wf_env_def e'_def
+                    by (smt (verit, best) Union_iff mem_Collect_eq)
+                  with \<open>\<S> e x = \<S> e y\<close> show ?thesis
+                    using False by (simp add: e'_def)
+                qed
+              next
+                assume sx: "\<S> e' x = \<S> e' y"
+                show "y \<in> \<S> e' x"
+                proof (cases "x \<in> cc")
+                  case True
+                  hence "\<S> e' x = cc"
+                    by (simp add: e'_def)
+                  moreover have "y \<in> cc"
+                  proof (rule ccontr)
+                    assume y: "y \<notin> cc"
+                    with \<open>\<S> e' x = cc\<close> sx have "\<S> e y = cc"
+                      by (simp add: e'_def)
+                    with \<open>wf_env e\<close> have "y \<in> cc"
+                      unfolding wf_env_def by metis
+                    with y show "False" ..
+                  qed
+                  ultimately show ?thesis 
+                    by simp
+                next
+                  case False
+                  hence "\<S> e' x = \<S> e x"
+                    by (simp add: e'_def)
+                  have "y \<notin> cc"
+                  proof
+                    assume y: "y \<in> cc"
+                    with \<open>\<S> e' x = \<S> e x\<close> sx have "\<S> e x = cc"
+                      by (simp add: e'_def)
+                    with \<open>wf_env e\<close> have "x \<in> cc"
+                      unfolding wf_env_def by metis
+                    with \<open>x \<notin> cc\<close> show "False" ..
+                  qed
+                  with sx \<open>\<S> e' x = \<S> e x\<close> 
+                  have "\<S> e y = \<S> e x"
+                    by (simp add: e'_def)
+                  with \<open>wf_env e\<close> have "y \<in> \<S> e x"
+                    unfolding wf_env_def by metis
+                  with \<open>\<S> e' x = \<S> e x\<close> show ?thesis
+                    by simp
+                qed
+              qed
+              hence "y \<in> \<S> e'' x \<longleftrightarrow> (\<S> e'' x = \<S> e'' y)"
+                by (simp add: e''_def)
+            }
+
+            moreover
+            have "\<forall>x \<in> set (stack e''). \<forall>y \<in> set (stack e'').
+                     x \<noteq> y \<longrightarrow> \<S> e'' x \<inter> \<S> e'' y = {}"
+            proof (clarify)
+              fix x y
+              assume "x \<in> set (stack e'')" "y \<in> set (stack e'')" "x \<noteq> y"
+              hence xy: "x \<in> set sfx" "y \<in> set sfx"
+                by (auto simp: e'_def e''_def)
+              show "\<S> e'' x \<inter> \<S> e'' y = {}"
+              proof (cases "x = hd sfx")
+                case True
+                with xy \<open>x \<noteq> y\<close> sfx have "y \<in> set (tl sfx)"
+                  by (metis list.exhaust_sel set_ConsD)
+                with True hd_sfx tl_sfx show ?thesis
+                  by (auto simp: e''_def)
+              next
+                case False
+                with xy sfx have "x \<in> set (tl sfx)"
+                  by (metis list.exhaust_sel set_ConsD)
+                show ?thesis
+                proof (cases "y = hd sfx")
+                  case True
+                  with \<open>x \<in> set (tl sfx)\<close> hd_sfx tl_sfx show ?thesis
+                    by (auto simp: e''_def)
+                next
+                  case False
+                  with xy sfx have "y \<in> set (tl sfx)"
+                    by (metis list.exhaust_sel set_ConsD)
+                  with \<open>x \<in> set (tl sfx)\<close> tl_sfx
+                  have "\<S> e'' x = \<S> e x \<and> \<S> e'' y = \<S> e y"
+                    by (auto simp: e''_def)
+                  with xy \<open>stack e = pfx @ sfx\<close> \<open>x \<noteq> y\<close> \<open>wf_env e\<close>
+                  show ?thesis
+                    by (auto simp: wf_env_def)
+                qed
+              qed
+            qed
+
+            moreover
+            have "\<forall>x. x \<notin> visited e'' \<longrightarrow> \<S> e'' x = {x}"
+            proof (clarify)
+              fix x
+              assume "x \<notin> visited e''"
+              hence "x \<notin> visited e"
+                by (simp add: e'_def e''_def)
+              moreover have "x \<notin> cc"
+              proof
+                assume "x \<in> cc"
+                then obtain n where
+                  "n \<in> set pfx \<union> {hd sfx}" "x \<in> \<S> e n"
+                  by (auto simp: cc_def)
+                with \<open>stack e = pfx @ sfx\<close> sfx \<open>wf_env e\<close> \<open>x \<notin> visited e\<close>
+                show "False"
+                  unfolding wf_env_def
+                  by (metis Un_iff list.set_sel(1) set_append singletonD subsetD)
+              qed
+              ultimately show "\<S> e'' x = {x}"
+                using \<open>wf_env e\<close> 
+                by (auto simp: wf_env_def e'_def e''_def)
+            qed
+
+            moreover
+            from s_equal \<open>wf_env e\<close>
+            have "\<Union> {\<S> e'' x | x. x \<in> set (stack e'')} = visited e'' - explored e''"
+              by (auto simp: wf_env_def e'_def e''_def)
+
+            moreover
+            have "\<forall>x y. x \<preceq> y in stack e'' \<longrightarrow> reachable y x"
+            proof (clarify)
+              fix x y
+              assume "x \<preceq> y in stack e''"
+              hence "x \<preceq> y in sfx"
+                by (simp add: e'_def e''_def)
+              with \<open>stack e = pfx @ sfx\<close> \<open>wf_env e\<close>
+              show "reachable y x"
+                unfolding wf_env_def by (metis precedes_append_left)
+            qed
+
+            moreover
+            from cc_scc \<open>wf_env e\<close>
+            have "\<forall>x. is_subscc (\<S> e'' x)"
+              by (auto simp: e''_def e'_def wf_env_def)
+
+            moreover
+            from \<open>wf_env e\<close>
+            have "\<forall>x \<in> explored e''. \<forall>y. reachable x y \<longrightarrow> y \<in> explored e''"
+              by (auto simp: e''_def e'_def wf_env_def)
+
+            moreover
+            from \<open>wf_env e\<close>
+            have "\<forall>S \<in> sccs e''. is_scc S"
+              by (auto simp: e''_def e'_def wf_env_def)
+
+            moreover
+            have "\<forall>x y. x \<preceq> y in stack e'' \<and> x \<noteq> y \<longrightarrow>
+                        (\<forall>u \<in> \<S> e'' x. \<not> reachable_avoiding u y (unvisited e'' x))"
+            proof (clarify)
+              fix x y u
+              assume xy: "x \<preceq> y in stack e''" "x \<noteq> y"
+                 and u: "u \<in> \<S> e'' x" "reachable_avoiding u y (unvisited e'' x)"
+              show "False"
+                sorry
+            qed
+
+            ultimately show ?thesis
+              unfolding wf_env_def by blast
+          qed
+
+          have "pre_dfss v e''"
+            sorry
+
+(*
+          moreover have "pre_dfss v e'"
+            sorry
       proof -
         have "wf_env e'"
         proof -
-          from e'_def \<open>wf_env e\<close> \<open>stack e = pfx @ sfx\<close>
-          have "distinct (stack e')" 
-               "set (stack e') \<subseteq> visited e'" 
-               "explored e' \<subseteq> visited e'"
-               "explored e' \<inter> set (stack e') = {}"
-            by (auto simp: wf_env_def)
 
           moreover
           from \<open>wf_env e\<close> have "\<forall>v w. w \<in> \<S> e v \<longleftrightarrow> (\<S> e v = \<S> e w)"
@@ -1955,16 +2058,54 @@ next
       ultimately show ?thesis
         unfolding pre_dfss_def by blast
     qed
+*)
 
-    moreover have "dfss v vs e = dfss v (vs - {w}) e'"
-      using False \<open>e' = unite v w e\<close> dfss.psimps dom notexplored vs_case w_def by force
-    moreover have "post_dfss v (vs - {w}) e' (dfss v (vs - {w}) e')"
-      using False \<open>e' = unite v w e\<close> calculation notexplored prepostdfss vs_case w_def
-      by (simp add: pre_dfss_def)
-    moreover have "post_dfss v vs e (dfss v (vs-{w}) e')" sorry
+          with prepostdfss vs_case \<open>e' = unite v w e\<close>  \<open>w \<notin> explored e\<close> \<open>w \<in> visited e\<close>
+          have post'': "post_dfss v e'' (dfss v e'')"
+            by (auto simp: w_def e''_def)
 
-    ultimately show ?thesis
-      by simp
+          moreover
+          have "\<forall>u \<in> visited e - {v}. vsuccs (dfss v e'') u = vsuccs e u"
+          proof
+            fix u
+            assume "u \<in> visited e - {v}"
+            have u: "vsuccs e' u = vsuccs e u" "u \<in> visited e'' - {v}"
+              sorry
+            with post'' have "vsuccs (dfss v e'') u = vsuccs e'' u"
+              by (auto simp: post_dfss_def)
+            with u show "vsuccs (dfss v e'') u = vsuccs e u"
+              by (simp add: e''_def)
+          qed
+
+          moreover
+          have "sub_env e (dfss v e'')"
+          proof -
+            have "sub_env e' e''"
+              by (auto simp: sub_env_def e''_def)
+            moreover
+            from post'' have "sub_env e'' (dfss v e'')"
+              by (simp add: post_dfss_def)
+            ultimately show ?thesis
+              using \<open>sub_env e e'\<close> sub_env_trans by metis
+          qed
+
+          moreover
+          have "\<exists>ns. stack e = ns @ (stack (dfss v e''))"
+            sorry
+
+          moreover
+          {
+            fix n
+            assume n: "n \<in> set (tl (stack (dfss v e'')))"
+            have "\<S> (dfss v e'') n = \<S> e n"
+              sorry
+          }
+
+          ultimately show ?thesis
+            by (auto simp: dfss post_dfss_def)
+        qed
+      qed
+    qed
   qed
 qed
 
